---
layout: post
title: Euler, "Elements of Algebra", Section II, Chapter 12. "Of the Expression of Irrational Powers by Infinite Series."
---

### Leonhard Euler, *Elements of Algebra* (*Vollständige Anleitung zur Algebra*)

#### Section II. "Of the different Methods of calculating Compound Quantities." Chapter 12. "Of the Expression of Irrational Powers by Infinite Series"

<span class="art">361</span> As we have shewn the method of finding any power
of the root $$a + b$$, however great the exponent may be, we
are able to express, generally, the power of $$a + b$$ whose
exponent is undetermined; for it is evident that if we
represent that exponent by $$n$$, we shall have by the rule already
given (**Art. 348** and the following):

$$
\begin{align}
(a+b)^n &= a^n + \frac{n}{1}a^{n-1}b+\frac{n}{1}\cdot \frac{n-1}{2} a^{n-2}b^2\\
&+\frac{n}{1}\cdot \frac{n-1}{2} \cdot \frac{n-2}{3} a^{n-3}b^3\\
&+\frac{n}{1}\cdot \frac{n-1}{2} \cdot \frac{n-2}{3} \cdot \frac{n-3}{4} a^{n-4}b^4
+\textrm{etc.}
\end{align}
$$


<span class="art">362</span> If the same power of the root $$a-b$$ were required,
we need only change the signs of the second, fourth,
sixth, etc. terms, and should have

$$
\begin{align}
(a-b)^n &= a^n - \frac{n}{1}a^{n-1}b+\frac{n}{1}\cdot \frac{n-1}{2} a^{n-2}b^2\\
&-\frac{n}{1}\cdot \frac{n-1}{2} \cdot \frac{n-2}{3} a^{n-3}b^3\\
&+\frac{n}{1}\cdot \frac{n-1}{2} \cdot \frac{n-2}{3} \cdot \frac{n-3}{4} a^{n-4}b^4
-\textrm{etc.}
\end{align}
$$

<span class="art">363</span> These formulas are remarkably useful, since they
serve also to express all kinds of radicals; for we have shown
that all irrational quantities may assume the form of powers
whose exponents are fractional, and that
$$\sqrt[2]{\vphantom{a}}a=a^{\frac{1}{2}}$$,
$$\sqrt[3]{\vphantom{a}}a=a^{\frac{1}{3}}$$,
$$\sqrt[4]{\vphantom{a}}a=a^{\frac{1}{4}}$$,
etc.: we have, therefore,

$$\sqrt[2]{\vphantom{(a+b)}}(a+b)=(a+b)^{\frac{1}{2}};
\; \sqrt[3]{\vphantom{(a+b)}}(a+b)=(a+b)^{\frac{1}{3}};
\; \sqrt[4]{\vphantom{(a+b)}}(a+b)=(a+b)^{\frac{1}{4}},
\; \textrm{etc.}$$

Consequently, if we wish to find the square root of $$a+b$$,
we have only to substitute for the exponent $$n$$ the fraction
½ in the general formula, **Art. 361**, and we shall have first, for
the coefficients,

$$\frac{n}{1}=\frac{1}{2}; \; \frac{n-1}{2}=-\frac{1}{4}; \;
\frac{n-2}{3}=-\frac{3}{6}; \; \frac{n-3}{4}=-\frac{5}{8}; \;
\frac{n-4}{5}=-\frac{7}{10}; \; \frac{n-5}{6}=-\frac{9}{12}.$$

Then $$a^n=a^{\frac{1}{2}}=\surd a$$ and $$a^{n-1}=\dfrac{1}{\surd a}$$;
$$a^{n-2}=\dfrac{1}{a\surd a}$$; $$a^{n-3}=\dfrac{1}{a^2 \surd a}$$, etc.
or we might express those powers of $$n$$ in the following manner:
$$a^n=\surd a$$; $$a^{n-1}=\dfrac{\surd a}{a}$$; $$a^{n-2}=\dfrac{a^n}{a^2}=\dfrac{\surd a}{a^2}$$;
$$a^{n-3}=\dfrac{a^n}{a^3} = \dfrac{\surd a}{a^3}$$;
$$a^{n-4}=\dfrac{a^n}{a^4} = \dfrac{\surd a}{a^4}$$, etc.

<span class="art">364</span> This being laid down, the square root of $$a + b$$ may
be expressed in the following manner:

$$\surd(a+b) = \surd a - \frac{1}{2}b \dfrac{\surd a}{a}-\frac{1}{2} \cdot \frac{1}{4} b^2 \dfrac{\surd a}{aa}
+\frac{1}{2}\cdot \frac{1}{4}\cdot \frac{3}{6}b^3 \dfrac{\surd a}{a^3}
-\frac{1}{2}\cdot \frac{1}{4}\cdot \frac{3}{6}\cdot \frac{5}{8} b^4 \dfrac{\surd a}{a^4},
\; \textrm{etc.}$$

<span class="art">365</span>




<span class="art">366</span>



<span class="art">367</span>



<span class="art">368</span>


<span class="art">369</span>


#### Editions

1. Leonhard Euler. *Elements of Algebra*. Translated by Rev. John Hewlett. Third Edition. Longmans, Hurst, Rees, Orme, and Co. London. 1822.
    - [Section II. Chapter 12. "Of the Expression of Irrational Powers by Infinite Series."](/assets/euler/en/II-12.pdf)
2. Leonhard Euler. *Vollständige Anleitung zur Algebra. Mit den Zusätzen von Joseph Louis Lagrange.* Herausgegeben von Heinrich Weber. B. G. Teubner. Leipzig and Berlin. 1911. Leonhardi Euleri Opera omnia. Series prima. Opera mathematica. Volumen primum.
    - [Erster Theil. Zweyter Abschnitt. Capitel 12. Von der Entwickelung der irrationalen Potestäten durch unendliche Reihen](/assets/euler/de/I-II-12.pdf)