---
layout: page
title: Chapter 4. "Of the Method of rendering Surd Quantities of the form ‚àö(ùëé+ùëèùë•+cùë•ùë•) rational."
part: II
chapter: 4
---

### Part {{ page.part}}. {{ page.title }}

<span class="art">38</span> It is required in the present case to determine tlie
values which are to be adopted for x, in order that the
formula a -\- bx -\- ex" may become a real square; and,
consequently, that a rational root of it may be assigned.
Now, the letters r/, b, and c, represent given numbers ; and
The determination of the unknown quantity depends chiefly
on the nature of these numbers; there being many cases in
which the solution becomes impossible. But even when it is
possible, we must content ourselves at first with being able to
assign rational values for the letter $$x$$, without requiring those
values also to be integer numbers; as this latter condition
produces researches altogether peculiar.

<span class="art">39</span> We suppose here that the formula extends no farther
than the second power of $$x$$; the higher dimensions require
different methods, which will be explained in their proper
places.

We shall observe first, that if the second power were not
in the formula, and $$c$$ were = 0, the problem would be attended with no difficulty;
for if $$\surd(a+bx)$$ were the given formula, and it were required to determine $$x$$,
so that $$a+bx$$ might be a square, we should only have to make $$a+bx=y^2$$,
whence we should immediately obtain $$x=\dfrac{y^2-a}{b}$$. Now,
whatever number we substitute here for $$y$$, the value of $$x$$ would always
be such, that $$a+bx$$ would be a square, and consequently,
$$\surd(a+bx)$$ would be a rational quantity.

<span class="art">40</span> We shall therefore begin with the formula $$\surd(1+x^2)$$;
that is to say, we are to find such values of $$x$$, that,
by adding unity to their squares, the sums may likewise be squares;
and as it is evident that those values of $$x$$ cannot be integers,
we must be satisfied with finding the fractions which express
them.

<span class="art">41</span> If we supposed $$1+x^2=y^2$$, since $$1+x^2$$ must be a square, we should have
$$x^2=y^2-1$$, and $$x=\surd(y^2-1)$$;
so that in order to find $$x$$ we should have to seek numbers
for $$y$$, whose squares, diminished by unity, would also leave
squares; and, consequently, we should be led to a question as
difficult as the former, without advancing a single step.

It is certain, however, that there are real fractions, which,
being substituted for $$x$$, will make $$1+x^2$$ a square; of
which we may be satisfied from the following cases:

1. If $$x=\frac{3}{4}$$, we have $$1+x^2=\frac{25}{16}$$; and consequently $$\surd(1+x^2)=\frac{5}{4}$$.
2. $$1+x^2$$ becomes a square likewise, if $$x=\frac{4}{3}$$, which gives $$\surd(1+x^2)=\frac{5}{3}$$.
3. If we make $$x=\frac{5}{12}$$, we obtain $$1+x^2=\frac{169}{144}$$, the square root of which is $$\frac{13}{12}$$.

But it is requii-ed to shew how to find these values of $$x$$,
and even all possible numbers of this kind.

<span class="art">42</span> There are two methods of doing this. The first requires us to make
$$\surd(1+x^2)=x+p$$;
from which supposition we have $$1+x^2=x^2+2px+p^2$$, where the square
$$x^2$$ destroys itself; so that we may express $$x$$ without a radical sign.
For, cancelling $$x^2$$ on both sides of the equation, we obtain $$2px+p^2=1$$; whence we find
$$x=\dfrac{1-p^2}{2p}$$; a quantity in which we may substitute for $$p$$ any number
whatever less than unity.

Let us therefore suppose $$p=\dfrac{m}{n}$$, and we have

$$x=\dfrac{1-\frac{m^2}{n^2}}{\frac{2m}{n}},$$

and if we multiply both terms of this fraction by $$n^2$$, we shall find $$x=\dfrac{n^2-m^2}{2mn}$$.

<span class="art">43</span> In order, therefore, that $$1 + x^2$$ may become a square,
we may take for $$m$$ and $$n$$ all possible integer numbers, and
in this manner find an infinite number of values for $$x$$.

Also, if we make, in general, $$x=\dfrac{n^2-m^2}{2mn}$$, we find,
by squaring,

$$1+x^2 = 1+\dfrac{n^4-2m^2n^2+m^4}{4m^2n^2},$$

or, by putting $$1=\dfrac{4m^2}{4m^2}$$ in the numerator,

$$1+x^2 = \dfrac{n^4+2m^2n^2+m^4}{4m^2n^2};$$

a fraction which is really a square, and gives

$$\surd(1+x^2) = \dfrac{n^2+m^2}{2mn}.$$

We shall exhibit, according to this solution, some of the
least values of $$x$$.

<table>
<tr>
<td>If \(n\) =</td>
<td>2,</td>
<td>3,</td>
<td>3,</td>
<td>4,</td>
<td>4,</td>
<td>5,</td>
<td>5,</td>
<td>5,</td>
<td>5,</td>
</tr>
<tr>
<td>and \(m\) =</td>
<td>1,</td>
<td>1,</td>
<td>2,</td>
<td>1,</td>
<td>3,</td>
<td>1,</td>
<td>2,</td>
<td>3,</td>
<td>4,</td>
</tr>
<tr>
<td>We have \(x\) =</td>
<td>¬æ,</td>
<td>‚Å¥‚ÅÑ‚ÇÉ,</td>
<td>‚Åµ‚ÅÑ‚ÇÅ‚ÇÇ,</td>
<td>¬π‚Åµ‚ÅÑ‚Çà,</td>
<td>‚Å∑‚ÅÑ‚ÇÇ‚ÇÑ,</td>
<td>¬π¬≤‚ÅÑ‚ÇÖ,</td>
<td>¬≤¬π‚ÅÑ‚ÇÇ‚ÇÄ,</td>
<td>‚Å∏‚ÅÑ‚ÇÅ‚ÇÖ,</td>
<td>‚Åπ‚ÅÑ‚ÇÑ‚ÇÄ.</td>
</tr>
</table>

<span class="art">44</span> We have, therefore, in general,

$$1+\dfrac{(n^2-m^2)^2}{(2mn)^2} = \dfrac{(n^2+m^2)^2}{(2mn)^2};$$

and, if we multiply this equation by $$(2mn)^2$$, we find

$$(2mn)^2+(n^2-m^2)^2 = (n^2+m^2)^2;$$

so that we know, in a general manner, two squares, whose
sum gives a new square. This remark will lead to the
solution of the following question:

To find two square numbers, whose sum is likewise a
square number.

We must have $$p^2+q^2=r^2$$; we have therefore only to make
$$p=2mn$$, and $$q=n^2-m^2$$, then we shall have
$$r=n^2+m^2$$.

Farther, as $$(n^2+m^2)^2 - (2mn)^2 = (n^2-m^2)^2$$, we may
also resolve the following question:

To find two squares, whose difference may also be a square
number.

Here, since $$p^2-q^2=r^2$$, we have only to suppose
$$p=n^2+m^2$$, and $$q=2mn$$, and we obtain $$r=n^2-m^2$$.
We might also make $$p=n^2+m^2$$, and $$q=n^2-m^2$$,
from which we should find $$r=2mn$$.

<span class="art">45</span> We spoke of two methods of giving the form of a
square to the formula $$1+x^2$$. The other is as follows:

If we suppose $$\surd(1+x^2)=1+\dfrac{mx}{n}$$, we shall have 

$$1+x^2 = 1+\dfrac{2mx}{n}+\dfrac{m^2x^2}{n^2};$$

subtracting 1 from both sides, we have

$$x^2 = \dfrac{2mx}{n} + \dfrac{m^2x^2}{n^2}.$$

This equation may be divided by $$x$$, so that we have

$$x=\dfrac{2m}{n}+\dfrac{m^2x}{n^2},$$

or $$n^2x=2mn+m^2x$$, whence we find $$x=\dfrac{2mn}{n^2-m^2}$$. Having found
this value of $$x$$, we have

$$1+x^2 = 1 + \dfrac{4m^2n^2}{n^4-2m^2n^2+m^4} = \dfrac{n^4+2m^2n^2+m^4}{n^4-2m^2n^2+m^4},$$

which is the square of $$\dfrac{n^2+m^2}{n^2-m^2}$$. Now, as we obtain from that, the
equation

$$1+\dfrac{(2mn)^2}{(n^2-m^2)^2} = \dfrac{(n^2+m^2)^2}{(n^2-m^2)^2},$$

we shall have, as before,

$$(n^2-m^2)^2 + (2mn)^2 = (n^2+m^2)^2;$$

that is, the same two squares, whose sum is also a square.

<span class="art">46</span>


<span class="art">47</span>

#### Editions

1. Leonhard Euler. *Elements of Algebra*. Translated by Rev. John Hewlett. Third Edition. Longmans, Hurst, Rees, Orme, and Co. London. 1822.
    - [Part {{ page.part}}. {{ page.title }}](/assets/euler/en/pt-II-4.pdf)
2. Leonhard Euler. *Vollst√§ndige Anleitung zur Algebra. Mit den Zus√§tzen von Joseph Louis Lagrange.* Herausgegeben von Heinrich Weber. B. G. Teubner. Leipzig and Berlin. 1911. Leonhardi Euleri Opera omnia. Series prima. Opera mathematica. Volumen primum.
    - [Zweyter Theil. Zweyter Abschnitt. Capitel 4. Von der Art diese irrationale Formeln $$\surd(a + bx + cxx)$$ rational zu machen](/assets/euler/de/II-II-4.pdf)