---
layout: post
title: Euler, "Elements of Algebra", Section IV, Chapter 11
---

### Leonhard Euler, *Elements of Algebra* (*Vollständige Anleitung zur Algebra*)

#### Section IV. "Of Algebraic Equations, and the Resolution of Them." Chapter 11. "Of the Resolution of Complete Equations of the Third Degree."

**719.** An equation of the third degree is called complete,
when, beside the cube of the unknown quantity, it contains
that unknown quantity itself, and its square: so that the
general formula for these equations, bringing all the terms
to one side, is

$$ax^3 \pm bx^2 \pm cx \pm d = 0.$$

And the purpose of this chapter is to show how we are to
derive from such equations the values of $$x$$, which are also
called the roots of the equation. We suppose, in the first
place, that every such an equation has three roots; since it
has been seen, in the last chapter, that this is true even with
regard to pure equations of the same degree.

**720.** We shall first consider the equation
$$x^3-6x^2+11x-6=0$$; and, since an equation of the second degree
may be considered as the product of two factors, we may
also represent an equation of tlie third degree by the product
of three tactors, which are in the present instance,

$$(x-1)(x-2)(x-3)=0;$$

since, by actually multiplying them, we obtain the given
equation; for $$(x-1)(x-2)$$ gives $$x^2-3x+2$$< and multiplying
this by $$x-3$$, we obtain $$x^3-6x^2+11x-6$$, which are the given
quantities, and which must be =0. Now, this happens, when the product
$$(x-1)(x-2)(x-3)=0$$; and, as it is sufficient for this purpose, that
one of the factors become =0, three different cases may give
this result, namely, when $$x-1=0$$, or $$x=1$$; secondly,
when $$x-2=0$$, or $$x=2$$; and thirdly, when $$x-3=0$$, or $$x=3$$.

We see immediately also, that if we substituted for $$x$$,
any number whatever beside one of the above three,
none of the three factors would become equal to 0; and,
consequently, the product would no longer be 0: which
proves that our equation can have no other root than these
three.

**721.** If it were possible, in every other case, to assign
the three factors of such an equation in the same manner,
we should immediately have its three roots. Let us, therefore, consider,
in a more general manner, these three factors, $$x-p$$, $$x-q$$, $$x-r$$.
Now, if we seek their product, the
first, multiplied by the second, gives
$$x^2-(p+q)x+pq$$, and this product, multiplied by $$x-r$$, makes

$$x^3-(p+q+r)x^2+(pq+pr+qr)x-pqr.$$

Hence, if this formula must become =0, it may happen in three cases:
the first is that in, in which $$x-p=0$$, or $$x=p$$;
and second is, when $$x-q=0$$, or $$x=q$$; the third is, when $$x-r=0$$,
or $$x=r$$.

**722.** Let us now represent the quantity found, by the
equation $$x^3-ax^2+bx-c=0$$. It is evident, in order that its
three roots may be $$x=p$$, $$x=q$$, $$x=r$$, that we must have,

1. $$a=p+q+r$$,
2. $$b=pq+pr+qr$$, and
3. $$c=pqr$$.

We perceive, from this, that the second term of the equation contains the sum of the three roots; that the third term
contains the sum of the products of the roots taken two by
two ; and lastly, that the fourth term consists of the product
of all the three roots multiplied together.

From this last property we may deduce an important
truth, which is, that an equation of the third degree can
have no other rational roots than the divisors of the last
term; for, since that term is the product of the three roots,
it must be divisible by each of them: so that when we wish
to find a root by trial, we immediately see what numbers
we are to use.

For example, let us consider the equation,
$$x^3=x+6$$, or $$x^3-x-6=0$$. Now, as this equation can have no
other rational roots than numbers which are factors of the
last term 6, we have only 1, 2, 3, 6, to try with, and the
result of these trials will be as follows:

If $$x=1$$, we have 1-1-6=-6.  
If $$x=2$$, we have 8-2-6=0.  
If $$x=3$$, we have 26-3-6=18.  
If $$x=6$$, we have 216-6-6=204.

Hence we see, that $$x=2$$ is one of the roots of the given equation;
and, showing this, it is easy to find the other two;
for $$x=2$$ being one of the roots $$x-2$$ is a factor of the equation,
adn as we have only to see the other factor by means of division as follows:







#### References

1. Leonhard Euler, *Elements of Algebra*, Translated by Rev. John Hewlett. Longmans, Hurst, Rees, Orme, and Co., London, 1822.
    - [Section IV. Chapter 11. "Of the Resolution of Complete Equations of the Third Degree."](/assets/euler/en/IV-11.pdf)
    - [Archive.org](https://archive.org/details/elementsofalgebr00euleuoft/)
3. Leonhard Euler. *Vollständige Anleitung zur Algebra. Mit den Zusätzen von Joseph Louis Lagrange.* Herausgegeben von Heinrich Weber. B. G. Teubner. Leipzig and Berlin. 1911. Leonhardi Euleri Opera omnia. Series prima. Opera mathematica. Volumen primum.
    - [Zweyter Theil. Erster Abschnitt. Capitel 11. Von der Auflösung der vollständigen cubischen Gleichungen](/assets/euler/de/II-I-11.pdf)
    - [Springer](https://link.springer.com/book/9783764314002)
2. Leonhard Euler, *Vollständige Anleitung zur Algebra. Zweyter Theil. Von Auflösung algebraischer Gleichungen und der unbestimmten Analytic*, Kays. Acad. der Wissenschaften, St. Petersburg, 1770.
    - [Deutsches Textarchiv](https://www.deutschestextarchiv.de/euler_algebra02_1770)