---
layout: post
title: Translating focus-directrix form quadratics to vertex form
topic: directrix
---

Let $$F=(h,t)$$ be the focus and $$y=d$$ be the directrix of the parabola. Let $$V=(h,k)$$ be the vertex with the parabola defined by $$y=\dfrac{1}{4f}(x-h)^2+k$$.

$$t=k+f$$ and $$d=k-f$$.

On the one hand, adding $$k=t-f$$ and $$k=d+f$$ gives $$2k=t+d$$, so

$$
k = \dfrac{t+d}{2}.
$$

On the other hand, adding $$f=t-k$$ and $$f=k-d$$ gives $$2f=t-d$$, so

$$
f=\dfrac{t-d}{2}.
$$

Therefore, given the focus $$F=(h,t)$$ and the directrix $$y=d$$, we have found that

$$
V=(h,k) = \left(h,\dfrac{t+d}{2} \right),
$$

$$
f = \dfrac{t-d}{2},
$$

and the vertex form of the parabola is

$$
\begin{align*}
y&=\dfrac{1}{4f}(x-h)^2+k\\
&=\dfrac{1}{2(t-d)}(x-h)^2+\dfrac{t+d}{2}
\end{align*}
$$

[Focus and directrix to vertex form](https://www.geogebra.org/calculator/znfcubaz)

<iframe src="https://www.geogebra.org/calculator/znfcubaz?embed" width="800" height="600" allowfullscreen style="border: 1px solid #e4e4e4;border-radius: 4px;" frameborder="0"></iframe>