---
layout: post
title: Parabola curvature
---

The radius of curvature of the curve $$(x,y(x))$$

$$
R=\dfrac{(1+[y'(x)]^2)^{\dfrac{3}{2}}}{\vert y''(x) \vert}
$$

$$
y(x)=a(x-h)^2+k
$$

$$
y'(x)=2a(x-h)
$$

$$
y''(x)=2a
$$


$$
R = \dfrac{(1+[2a(x-h)]^2)^{\dfrac{3}{2}}}{\vert 2a \vert}
$$

At the vertex $$(h,k)$$ the radius of curvature is

$$
R = \dfrac{1}{\vert 2a\vert}
$$


Focal length is $$\vert f \vert$$ where

$$
f=\dfrac{1}{4a}
$$

$$
\vert 2f\vert = \dfrac{1}{\vert 2a \vert} = R
$$

Thus

$$
R = 2 \vert f \vert, \quad \vert f \vert = \dfrac{R}{2}
$$


[HyperPhysics: Mirror Equation](http://hyperphysics.phy-astr.gsu.edu/hbase/geoopt/mireq.html)