---
layout: post
title: Rational function equation
math: \\(\frac{1}{x-2}+\frac{x-1}{x+2}=1\\)
---

$$
\begin{gather}
\frac{1}{x-2}+\frac{x-1}{x+2}=1\\
\frac{x+2}{x+2} \frac{1}{x-2}+\frac{x-2}{x-2} \frac{x-1}{x+2}=1\\
\frac{(x+2)\cdot 1}{(x+2)(x-2)} + \frac{(x-2)(x-1)}{(x-2)(x+2)}=1\\
\frac{x+2}{(x+2)(x-2)}+\frac{x^2-x-2x+2}{(x+2)(x-2)}=1\\
\frac{x+2}{(x+2)(x-2)}+\frac{x^2-3x+2}{(x+2)(x-2)}=1\\
\frac{x^2+x-3x+2+2}{(x+2)(x-2)}=1\\
\frac{x^2-2x+4}{(x+2)(x-2)}=1\\
x^2-2x+4 = (x+2)(x-2)\\
x^2-2x+4 = x^2-2x+2x-4\\
x^2-2x+4 = x^2-4\\
-2x+4=-4\\
-2x=-8\\
x=4
\end{gather}
$$

[Symbolab](/assets/symbolab/rationalA.pdf)