---
layout: post
title: Euler, "Elements of Algebra", Section IV, Chapter 8
---

### Leonhard Euler, *Elements of Algebra* (*Vollständige Anleitung zur Algebra*)

#### Section IV. "Of Algebraic Equations, and the Resolution of Them." Chapter 8. "Of the Extraction of the Square Roots of Binomials."

**669.** By a *binomials* we mean a quantity composed of
two parts, which are either both affected by the sign of the
square root, or of which one, at least, contains that sign.

For this reason 3+√5 is a binomial, and likewise
√8+√3; and it is indifferent whether the two terms be
joined by the sign + or by the sign - . So that 3 - √5
and 3 + √5 are both binomials.

**670.** The reason that these binomials deserve particular
attention is, that in the resolution of quadratic equations we
are always brought to quantities of this form, when the resolution cannot be performed. For example, the equation

$$x^2=6x-4$$

gives $$x = 3 + \surd 5$$.

It is evident, therefore, that such quantities must often
occur in algebraic calculations; for which reason, we have
already carefully shewn how they are to be treated in the
ordinary operations of addition, subtraction, multiplication,
and division, but we have not been able till now to show
how their square roots are to be extracted; that is, so far as
that extraction is possible; for when it is not, we must be
satisfied with affixing to the quantity another radical sign.
Thus, the square root of 3+√2 is written $$\sqrt{3 + \surd 2}$$;
$$\surd(3+\surd 2)$$.

**671.** It must here be observed, in the first place, that the
squares of such binomials are also binomials of the same
kind; in which also one of the terms is always rational.

For, if we take the square of $$a+\surd b$$. we shall obtain
$$(a^2+b)+2a\surd b$$. If therefore it were required reciprocally
to take the root of the quantity $$(a^2+b)+2a\surd b$$,
we should find it to be $$a+\surd b$$, and it is undoubtedly much easier to
form an idea of it in this manner, than if we had only put
the sign √ before the quantity.

**672.** It is chiefly required, therefore, to assign a character,
which may, in all cases, point out whether such a square
root exists or not; for which purpose we shall begin with an
easy quantity, requiring whether we can assign, in the sense
that we have explained, the square root of the binomial
5+2√6.

Suppose, therefore, that this root is $$\surd x+\surd y$$; the square of it
is $$(x+y)+2\surd xy$$, which must be equal to
the quantity 5+2√6. Consequently, the rational part $$x+y$$ must be equal to 5, and the irrational part
$$2\surd xy$$ must be equal to 2√6; which last equality gives $$\surd xy=\surd 6$$.
Now, since $$x+y=5$$,  we have $$y=5-x$$, and
this value substituted in the equation $$xy=6$$, produces
$$5x-x^2=6$$, or $$x^2=5x-6$$; therefore

$$x=\frac{5}{2}+\sqrt{\vphantom{\left( \frac{25}{4}-\frac{24}{4}\right)}}\left( \frac{25}{4}-\frac{24}{4}\right)=\frac{5}{2}+\frac{1}{2}=3.$$

So that $$x=3$$ and $$y=2$$; whence we
conclude, that the square root of 5+2√6 is √3+√2.

**673.** As we have here found the two equations, $$x + y = 5$$,
and $$xy = 6$$, we shall give a particular method for obtaining
the values of $$x$$ and $$y$$.

Since $$x+y = 5$$, by squaring, $$x^2+2xy+y^2= 25$$; and
as we know that $$x^2- 2xy + y^2$$ is the square of $$x - y$$, let
us subtract from $$x^2+2xy+y^2= 25$$, the equation $$xy=6$$,
taken four times, or $$4xy=24$$, in order to have
$$x^2-2xy+y^2=1$$; whence by extraction we have $$x-y=1$$; and as
$$x+y=5$$, we shall easily find $$x=2$$ and $$y=3$$:
wherefore, the square root of 5+2√6 is √3+√2.

**674.** Let us now consider the general binomial $$a+\surd b$$,
and supposing its square root to be $$\surd x+\surd y$$, we shall
have the equation

$$(x+y)+2\surd xy=a+\surd b;$$

so that $$x+y=a$$, and $$2\surd xy=\surd b$$, or $$4xy=b$$;
subtracting
this square from the square of the equation $$x+y=a$$, that
is, from $$x^2+2xy+y^2=a^2$$, there remains
$$x^2-2xy+y^2=a^2-b$$, the square root of which is
$$x-y=\surd(a^2-b)$$. Now, $$x+y=a$$; we have therefore
$$x=\dfrac{a+\surd(a^2-b)}{2}$$
and
$$y=\dfrac{a-\surd(a^2-b)}{2}$$;
consequently, the square root required of
$$a+\surd b$$ is

$$\dfrac{a+\surd(a^2-b)}{2}+\dfrac{a-\surd(a^2-b)}{2}.$$

**675.** We admit that this expression is more complicated
than if we had simply put the radical sign √ before the
given binomial $$a+\surd b$$, and written it
$$\surd(a+\surd b)$$:
but
the above expression may be greatly simplified when the
numbers
$$a$$ and $$b$$ are such, that $$a^2-b$$ is a square;
since
then the sign √, which is under the radical, disappears.
We see also, at the same time, that the square root of the
binomial $$a+\surd b$$ cannot be conveniently extracted, except
when $$a^2-b=c^2$$; for in this case the square root required is

$$
\sqrt{\vphantom{\left(\frac{a+c}{2}\right)}} \left(\frac{a+c}{2}\right) +
\sqrt{\vphantom{\surd\left(\frac{a-c}{2}\right)}}\left(\frac{a-c}{2}\right):
$$

but if $$a^2-b$$
is not a perfect square, we cannot express the square root of $$a+\surd b$$
more simply, than by putting the radical sign √ before it.

**676.** The condition, therefore, which is requisite, in order
that we may express the square root of a binomial $$a+\surd b$$
in a more convenient form, is, that $$a^2-b$$ be a square;
and
if we represent that square by $$c^2$$, we shall have for the
square root in question $$\sqrt{\vphantom{\left(\frac{a+c}{2}\right)}} \left(\frac{a+c}{2}\right) +
\sqrt{\vphantom{\surd\left(\frac{a-c}{2}\right)}}\left(\frac{a-c}{2}\right)$$;
for,  by squaring this quantity, we get

$$a-2\sqrt{\vphantom{\left(\frac{a^2-c^2}{4}\right)}}\left(\frac{a^2-c^2}{4}\right);$$

now, since $$c^2=a^2-b$$, and consequently $$a^2-c^2=b$$, the same square is found
equal to

$$a-2\sqrt{\vphantom{\frac{b}{4}}} \frac{b}{4} = a-\dfrac{2\surd b}{2} = a-\surd b.$$

**677.** When it is required, therefore, to extract the square
root of a binomial, as $$a \pm \surd b$$,
the rule is, to subtract from the square $$a^2$$
of the rational part the square $$b$$
of the irrational part, to take the square root of the remainder, and
calling that root $$c$$, to write for the root required

$$
\sqrt{\vphantom{\left(\frac{a+c}{2}\right)}} \left(\frac{a+c}{2}\right) \pm
\sqrt{\vphantom{\surd\left(\frac{a-c}{2}\right)}}\left(\frac{a-c}{2}\right):
$$

**678.** If the square root of 2+√3 were required, we
should have $$a=2$$ and $$\surd b=\surd 3$$; wherefore
$$a^2-b=c=1$$; so that by the formula just given, the root sought
equals √³⁄₂+√½.

Let it be required to find the square root of the binomial
11+6√2. Here we shall have $$a=11$$, and $$\surd b=6\surd 2$$;
consequently, $$b=36\cdot 2=72$$, and $$a^2-b=49$$, which
gives $$c=7$$; and hence we conclude, that the square root
of 11+6√2 is √9+√2, or 3+√2.

Required the square root of 11+2√30. Here $$a=11$$, $$\surd b = 2\surd 30$$;
consequently, $$b=4\cdot 30=120$$, $$a^2-b=1$$, and $$c=1$$;
therefore the root required is √6+√5.

**679.** This rule also applies, even when the binomial contains imaginary, or impossible quantities.

Let there be proposed, for example, the binomial 1+4√-3. First, we shall have
$$a=1$$ and $$\surd b = 4\surd -3$$, that is to say,
$$b=-48$$, and $$a^2-b=49$$; therefore
$$c=7$$, and consequently the square root required is
√4+√-3=2+√-3.

Again, let there be given -½+½√-3. First, we have $$a=-\frac{1}{2}$$;
$$\surd b = \frac{1}{2}\surd -3$$,
and $$b=\frac{1}{4}\cdot -3=-\frac{3}{4}$$;
whence $$a^2-b=\frac{1}{4}+\frac{3}{4}=1$$, and $$c=1$$;
and the result
required is 
$$\surd \frac{1}{4}+\surd -\frac{3}{4}=\frac{1}{2}+\frac{\surd -3}{2}$$, or
$$\frac{1}{2}+\frac{1}{2}\surd -3$$.

Another remarkable example is that in which it is required
to find the square root of 2√-1. As there is here no
rational part, we shall have $$a=0$$. Now, $$\surd b=2\surd -1$$,
and $$b=-4$$; wherefore $$a^2-b=4$$ and $$c=2$$;
consequently, the square root required is
√1+√-1=1+√-1, and the square of this quantity is found to be
1+2√-1-1=2√-1.

**680.** Suppose now we have such an equation as
$$x^2=a^2 \pm b$$, and that $$a^2-b=c^2$$;
we conclude from this, that
the value of

$$
x=\sqrt{\vphantom{\left(\frac{a+c}{2}\right)}} \left(\frac{a+c}{2}\right) \pm
\sqrt{\vphantom{\surd\left(\frac{a-c}{2}\right)}}\left(\frac{a-c}{2}\right),
$$

which may be useful
in many cases.

For example, if $$x^2=17+12\surd 2$$, and we shall have
$$x=3+\surd 8=3+2\surd 2$$.

**681.** This case occurs most frequently in the resolution of
equations of the fourth degree, such as
$$x^4=2ax^2+d$$. For,
if we suppose $$x^2=y$$, we have $$x^4=y^2$$,
which reduces the
given equation to $$y^2=2ay+d$$,
and from this we find
$$y=a \pm \surd(a^2+d)$$, therefore,
$$x^2=a \pm \surd(a^2+d)$$,
and
consequently we have anoth.er evolution to perform. Now,
since $$\surd b=\surd(a^2+d)$$, we have $$b=a^2+d$$,
and $$a^2-b=-d$$; if, therefore, $$-d$$ is a square,
as $$c^2$$, that is to say, $$d=-c^2$$,
we may assign the root required.

Suppose, in reality, that $$d=-c^2$$;
or that the proposed
equation of the fourth degree is $$x^4=2ax^2-c^2$$,
we shall then
find that

$$
x=\sqrt{\vphantom{\left(\frac{a+c}{2}\right)}} \left(\frac{a+c}{2}\right) \pm
\sqrt{\vphantom{\surd\left(\frac{a-c}{2}\right)}}\left(\frac{a-c}{2}\right).
$$

**682.** We shall illustrate what we have just said by some
examples.

***Example 1.*** Required two numbers, whose product may be 105,
and whose squares may together make 274.

Let us represent those two numbers by $$x$$ and $$y$$; we shall
then have the two equations,

$$xy=105$$  
$$x^2+y^2=274.$$

The first gives $$y=\dfrac{105}{x}$$,
and this value of $$y$$ being substituted in the second equation, we have

$$x^2+\dfrac{105^2}{x^2}=274.$$

Wherefore $$x^4+105^2=274x^2$$, or
$$x^4=274x^2-105^2$$.

If we now compare this equation with that in the preceding article, we have
$$2a=274$$, and $$-c^2=-105^2$$; consequently, $$c=105$$,
and $$a=137$$. We therefore find

$$
x=\sqrt{\vphantom{\left(\frac{137+105}{2}\right)}} \left(\frac{137+105}{2}\right) \pm
\sqrt{\vphantom{\surd\left(\frac{137-105}{2}\right)}}\left(\frac{137-105}{2}\right)
=11 \pm 4.
$$

Whence $$x = 15$$, or $$x - 7$$. In the first case, $$y=7$$, and in
the second case, $$y=15$$; whence the two numbers sought are
15 and 7.

**683.** It is proper, however, to observe, that this calculation may be performed
much more easily in another way. For, since
$$x^2+2xy+y^2$$ and $$x^2-2xy+y^2$$ are squares,
and since the values of $$x^2+y^2$$ and $$xy$$ are given,
we have
only to take the double of this last quantity, and then to add
and subtract it from the first, as follows:
$$x^2+y^2=274$$; to which if we add $$2xy=210$$, we have
$$x^2+2xy+y^2=484$$, which gives $$x+y=22$$.

But subtracting $$2xy$$, there remains
$$x^2-2xy+y^2=64$$, whence we find $$x-y=8$$.

So that $$2x=30$$, and $$2y=14$$; consequently, $$x = 15$$
and $$y=7$$.

The following general question is resolved by the same
method.

***Example 2.*** Required two numbers, whose product may be $$m$$, and
the sum of the squares $$n$$.

If those numbers are represented by $$x$$ and $$y$$, we have the
two following equations:

$$xy=m$$  
$$x^2+y^2=n.$$

Now, $$2xy=2m$$, being added to $$x^2+y^2-n$$,
we have $$x+2+2xy+y^2=n+2m$$, and consequently,

$$x+y=\surd(n+2m).$$

But subtracting $$2xy$$, there remains $$x^2-2xy+y^2=n-2m$$,
whence we get $$x-y=\surd(n-2m)$$; we have,
therefore,

$$x=\frac{1}{2}\surd(n+2m)+\frac{1}{2}\surd(n-2m);$$

and

$$y=\frac{1}{2}\surd(n+2m)+\frac{1}{2}\surd(n-2m).$$

**684.** ***Example 3.*** Required two numbers, such, that their product
may be 35, and the difference of their squares 24.

Let the greater of the two numbers be $$x$$, and the less $$y$$:
then we shall have the two equations

$$xy=35,$$  
$$x^2-y^2=24;$$

and as we have not the same advantages here, we shall proceed in the usual manner.
Here, the first equation gives $$y=\dfrac{35}{x}$$,
and, substituting this value of $$y$$ in the second, we
have $$x^2-\dfrac{1225}{x^2}=24$$; or $$x^4=24x^2+1225$$.
Now, the second member of this equation being affected by the sign +,
we cannot make use of the formula already given, because
having $$c^2=-1225$$, $$c$$ would become imaginary.

Let us therefore make $$x^2=z$$; we shall then have
$$z^2=24z+1225$$, whence we obtain

$$z=12 \pm \surd(144+1225), \: \textrm{or,} \: z=12 \pm 37;$$

consequently, $$x^2=12 \pm 37$$; that is to say,
either $$x^2=49$$ or $$x^2=-25$$.

If we adopt the first value, we have $$x=7$$ and $$y=5$$.

The second value gives $$x=\surd -25$$; and, since $$xy=35$$,
we have

$$y=\frac{35}{\surd -25} =
\sqrt{\vphantom{\frac{1225}{-25}}} \frac{1225}{-25}=\surd -49.$$

**685.** We shall conclude this chapter with the following
question.

***Example 4.*** Required two numbers, such, that their sum, their
product, and the difference of their squares, may be all
equal.

Let $$x$$ be the greater of the two numbers, and $$y$$ the less;
then the three following expressions must be equal to one
another: namely, (I) the sum, $$x+y$$; (II) the product, $$xy$$; and
(III) the difference of the squares, $$x^2-y^2$$. If we compare the
first with the second, we have $$x+y=xy$$; which will give
a value of $$x$$: for
$$y = xy - x = x(y-1)$$,
and $$x=\dfrac{y}{y-1}$$.
Consequently, 

$$x+y=\dfrac{y}{y-1}+y=\dfrac{y^2}{y-1},$$

and $$xy=\frac{y^2}{y-1}$$, that is to say, the sum is equal to the product; and to this
also the difference of the squares ought to be equal. Now,



#### References

1. Leonhard Euler, *Elements of Algebra*, Translated by Rev. John Hewlett. Longmans, Hurst, Rees, Orme, and Co., London, 1822.
    - [Section IV. Chapter 8. "Of the Extraction of the Square Roots of Binomials."](/assets/euler/en/IV-8.pdf)
    - [Archive.org](https://archive.org/details/elementsofalgebr00euleuoft/)
3. Leonhard Euler. *Vollständige Anleitung zur Algebra. Mit den Zusätzen von Joseph Louis Lagrange.* Herausgegeben von Heinrich Weber. B. G. Teubner. Leipzig and Berlin. 1911. Leonhardi Euleri Opera omnia. Series prima. Opera mathematica. Volumen primum.
    - [Zweyter Theil. Erster Abschnitt. Capitel 8. Von der Ausziehung der Quadrat-Wurzeln aus Binomien](/assets/euler/de/II-I-8.pdf)
    - [Springer](https://link.springer.com/book/9783764314002)
2. Leonhard Euler, *Vollständige Anleitung zur Algebra. Zweyter Theil. Von Auflösung algebraischer Gleichungen und der unbestimmten Analytic*, Kays. Acad. der Wissenschaften, St. Petersburg, 1770.
    - [Deutsches Textarchiv](https://www.deutschestextarchiv.de/euler_algebra02_1770)