---
layout: page
title: Chapter 6. "Of the Squares of Compound Quantities."
part: I
section: II
chapter: 6
---

### Part {{ page.part }}. Section {{ page.section }}. {{ page.title }}

<span class="art">306</span> When it is required to find the square of a compound quantity, we have only
to multiply it by itself, and the product will be the square required.

For example, the square of $$a + b$$ is found in the following
manner:

$$
\begin{array}{rrr}
a&+b&\\
a&+b&\\
\hline
a^2&+ab&\\
&+ab&+b^2\\
\hline
a^2&+2ab&+b^2
\end{array}
$$

<span class="art">307</span> So that when the root consists of two terms added
together, as $$a + b$$, the square comprehends, 1st, the squares
of each term, namely, $$a^2$$ and $$b^2$$; and 2nd, twice the product of the
two terms, namely, $$2ab$$: so that the sum $$a^2+2ab+b^2$$
is the square of $$a+b$$. Let, for example, $$a=10$$,
and $$b=3$$; that is to say, let it be required to find the square
of 10 + 3, or 13, and we shall have 100 + 60 + 9, or 169.

<span class="art">308</span> We may easily find, by means of this formula, the
squares of numbers, however great, if we divide them into
two parts. Thus, for example, the square of 57, if we consider that this number
is the same as 50 + 7, will be found = 2500 + 700 + 49 = 3249.

<span class="art">309</span> Hence it is evident, that the square of $$a + 1$$ will be
$$a^2+2a+1$$: and since the square of $$a$$ is $$a^2$$, we find the
square of $$a+1$$ by adding to that square $$2a+1$$; and it
must be observed, that this $$2a+1$$ is the sum of the two
roots $$a$$ and $$a+1$$.

Thus, as the square of 10 is 100, that of 11 will be 100 + 21:
the square of 57 being 3249, that of 58 is 3249 + 115 = 3364; the square of
59 = 3364 + 117 = 3481; the square of 60 = 3481 + 119 = 3600, etc.

<span class="art">310</span> The square of a compound quantity, as $$a + b$$, is
represented in this manner $$(a+b)^2$$. We have therefore

$$(a+b)^2=a^2+2ab+b^2,$$

whence we deduce the following equations:

$$
\begin{gather}
(a+1)^2=a^2+2a+1;\\
(a+2)^2=a^2+4a+4;\\
(a+3)^2=a^2+6a+9;\\
(a+4)^2=a^2+8a+16;\\
\textrm{etc.}
\end{gather}
$$

<span class="art">311</span> If the root be $$a - b$$, the square of it is
$$a^2 - 2ab + b^2$$, which contains also the squares of the two terms, but in
such a manner, that we must take from their sum twice the
product of those two terms. Let, for example, $$a = 10$$, and
$$b = - 1$$, then the square of 9 will be found equal to
100 - 20 + 1 = 81.

<span class="art">312</span> Since we have the equation

$$(a-b)^2=a^2-2ab+b^2,$$

we shall have $$(a - 1)^2 = a^2 - 2a + 1$$. The square of
$$a - 1$$ is found, therefore, by subtracting from $$a^2$$ the sum of
the two roots $$a$$ and $$a - 1$$, namely, $$2a - 1$$. Thus, for
example, if $$a = 50$$, we have $$a^2 = 2500$$, and $$2a - 1 = 99$$;
therefore $$49^2 = 2500 - 99 = 2401$$.

<span class="art">313</span> What we have said here may be also confirmed and
illustrated by fractions; for if we take as the root
⅗ + ⅖ = 1, the square will be, ⁹⁄₂₅ + ⁴⁄₂₅ + ¹²⁄₂₅ = 1.

Farther, the square of ½ - ⅓ = ⅙ will be
¼ - ⅓ + ⅑ = ¹⁄₃₆.

<span class="art">314</span> When the root consists of a greater number of terms,
the method of determining the square is the same. Let us
find, for example, the square of $$a + b + c$$:

$$
\begin{array}{rrrrrr}
a&+b&+c&&&\\
a&+b&+c&&&\\
\hline
a^2&ab&+ac&&&\\
&&ab&+b^2&+bc&\\
&&&+ac&+bc&+c^2\\
\hline
a^2&+2ab&+2ac&+b^2&+2bc&+c^2\\
\end{array}
$$

We see that it contains, first, the square of each term of
the root, and beside that, the double products of those terms
multiplied two by two.

<span class="art">315</span> To illustrate this by an example, let us divide the
number 256 into three parts, 200+50+6; its square
will then be composed of the following parts:

$$
\begin{array}{rcl}
200^2&=&40000\\
50^2&=&2500\\
6^2&=&36\\
2(50 \cdot 200) &=& 20000\\
2(6 \cdot 200) &=& 2400\\
2(6 \cdot 50) &=& 600\\
\hline
65536&=&256\cdot 256
\end{array}
$$

<span class="art">316</span> When some terms of the root are negative, the
square is still found by the same rule; only we must be
careful what signs we prefix to the double products. Thus,

$$(a-b-c)^2 = a^2 + b^2 + c^2 - 2ab - 2ac + 2bc;$$

and if
we represent the number 256 by 300-40-4, we shall
have,

$$
\begin{array}{r}
\textrm{Positive Parts.}\\
300^2=90000\\
400^2=16000\\
2(40\cdot 4)=320\\
4^2=16\\
\hline
91936
\end{array}
$$

$$
\begin{array}{r}
\textrm{Negative Parts.}\\
2(40 \cdot 300)=24000\\
2(4 \cdot 300) = 2400\\
\hline
-26400
\end{array}
$$

$$
\begin{array}{r}
91936\\
-26400\\
\hline
65536
\end{array}
$$

the square of 256 as before.

#### Editions

1. Leonhard Euler. *Elements of Algebra*. Translated by Rev. John Hewlett. Third Edition. Longmans, Hurst, Rees, Orme, and Co. London. 1822.
    - [Part {{ page.part }}. Section {{ page.section }}. {{ page.title }}](/EulerAlgebra/en/II-6.pdf)
2. Leonhard Euler. *Vollständige Anleitung zur Algebra. Mit den Zusätzen von Joseph Louis Lagrange.* Herausgegeben von Heinrich Weber. B. G. Teubner. Leipzig and Berlin. 1911. Leonhardi Euleri Opera omnia. Series prima. Opera mathematica. Volumen primum.
    - [Erster Theil. Zweyter Abschnitt. Capitel 6. Von den Quadraten der zusammengesetzten Größen](/EulerAlgebra/de/I-II-6.pdf)