---
layout: page
title: Chapter 7. "Of the Extraction of the Roots of Polygon Numbers."
part: I
section: IV
chapter: 7
---

### Part {{ page.part }}. Section {{ page.section }}. {{ page.title }}

<span class="art">656</span> We have shown, in a preceding chapter (Section III, Chapter 5. "Of Figurate, or Polygonal Numbers."), how
polygonal numbers are to be found; and what we then called
a **side**, is also called a **root**. If, therefore, we represent the
root by $$x$$, we shall find the following expressions for all
polygonal numbers

<table>
<tbody>
  <tr>
    <td>3-gon</td>
    <td>\( \dfrac{x^2+x}{2} \)</td>
  </tr>
  <tr>
    <td>4-gon</td>
    <td>\( x^2 \)</td>
  </tr>
  <tr>
    <td>5-gon</td>
    <td>\( \dfrac{3x^2-x}{2} \)</td>
  </tr>
  <tr>
    <td>6-gon</td>
    <td>\( 2x^2-x \)</td>
  </tr>
  <tr>
    <td>7-gon</td>
    <td>\( \dfrac{5x^2-3x}{2} \)</td>
  </tr>
  <tr>
    <td>8-gon</td>
    <td>\( 3x^2-2x \)</td>
  </tr>
  <tr>
    <td>9-gon</td>
    <td>\( \dfrac{7x^2-5x}{2} \)</td>
  </tr>
  <tr>
    <td>10-gon</td>
    <td>\( 4x^2-3x \)</td>
  </tr>
  <tr>
    <td>\(n\)-gon</td>
    <td>\( \dfrac{(n-2)x^2-(n-4)x}{2} \)</td>
  </tr>
</tbody>
</table>

<span class="art">657</span> We have already shown, that it is easy, by means of
these formulae, to find, for any given root, any polygon
number required: but when it is required reciprocally to
find the side, or the root of a polygon, the number of whose
sides is known, the operation is more difficult, and always
requires the solution of a quadratic equation; on which account the subject deserves,
in this place, to be separately considered. In doing this we shall proceed regularly,
beginning with the triangular numbers, and passing from them
to those of a greater number of angles.

<span class="art">658</span> Let therefore 91 be the given triangular number,
the side or root of which is required.

If we make this root =$$x$$, we must have
$$\dfrac{x^2+x}{2}=91$$; or $$x^2+x=182$$, and $$x^2=-x+182$$; consequently,

$$x=-\frac{1}{2}+\surd\left(\frac{1}{4}+182\right) = -\frac{1}{2} + \surd\left(\frac{729}{4}\right)
=-\frac{1}{2} + \frac{27}{2}=13;$$

from which we conclude, that the triangular root required is
13; for the triangle of 13 is 91.

<span class="art">659</span> But, in general, let $$a$$ be the given triangular number,
and let its root be required.

Here if we make it $$=x$$, we have $$\dfrac{x^2+x}{2}=a$$, or $$x^2+x=2a$$; therefore, $$x^2=-x+2a$$, and by
the rule $$x=-\frac{1}{2} +\surd\left(\frac{1}{4}+2a\right)$$, or $$x=\dfrac{-1 + \surd(8a+1)}{2}$$.

This result gives the following rule: To find a triangular root, we must multiply the given triangular number
by 8, add 1 to the product, extract the root of the sum,
subtract 1 from that root, and lastly, divide the remainder
by 2.

<span class="art">660</span> So that all triangular numbers have this property;
that if we multiply them by 8, and add unity to the product,
the sum is always a square; of which the following small
Table furnishes some examples:

<div style="overflow-x:auto;">
<table>
<tbody>
  <tr>
    <td>Triangles</td>
    <td>1</td>
    <td>3</td>
    <td>6</td>
    <td>10</td>
    <td>15</td>
    <td>21</td>
    <td>28</td>
    <td>36</td>
    <td>45</td>
    <td>55</td>
    <td>etc.</td>
  </tr>
  <tr>
    <td>8 times + 1 =</td>
    <td>9</td>
    <td>25</td>
    <td>49</td>
    <td>81</td>
    <td>121</td>
    <td>169</td>
    <td>225</td>
    <td>289</td>
    <td>361</td>
    <td>441</td>
    <td>etc.</td>
  </tr>
</tbody>
</table>
</div>

If the given number a does not answer this condition, we
conclude, that it is not a real triangular number, or that no
rational root of it can be assigned.

<span class="art">661</span> According to this rule, let the triangular root of 210
be required; we shall have $$a = 210$$, and $$8a + 1 = 1681$$,
the square root of which is 41; whence we see, that
the number 210 is really triangular, and that its root is
$$\dfrac{41-1}{2}=20$$. But if 4 were given as the triangular number,
and its root were required, we should find it
$$=\dfrac{\surd 33}{2}-\dfrac{1}{2}$$, and consequently irrational.
However, the triangle of this root, $$\dfrac{\surd 33}{2}-\dfrac{1}{2}$$,
may be found in the following manner:

Since $$x=\dfrac{\surd 33-1}{2}$$, we have $$x^2=\dfrac{17-\surd 33}{2}$$, and adding
$$x=\dfrac{\surd 33-1}{2}$$ to it, the sum is $$x^2+x=\frac{16}{2}=8$$. Consequently, the
triangle, or the triangular number, is $$\dfrac{x^2+x}{2}=4$$.

<span class="art">662</span> The quadrangular numbers being the same as
squares, they occasion no difficulty. For, supposing the
given quadrangular number to be $$a$$, and its required
root $$a$$;, we shall have $$x^2=a$$, and consequently, $$x=\surd a$$;
so that the square root and the quadrangular root are the
same thing.

<span class="art">663</span> Let us now proceed to pentagonal numbers.

Let 22 be a number of this kind, and $$x$$ its root; then, by
the third formula, we shall have $$\dfrac{3x^2-x}{2}=22$$, or
$$3x^2-x=44$$, or $$x^2=\frac{1}{3}x+\frac{44}{3}$$; from which
we obtain, $$x=\frac{1}{6}+\surd\left(\frac{1}{16}+\frac{44}{3}\right)$$,
or

$$x=\dfrac{1+\surd (529)}{6} = \frac{1}{6}+\frac{23}{6}=4;$$

and consequently 4 is the pentagonal root of the number 22.

<span class="art">664</span> Let the following question be now proposed: the
pentagon $$a$$ being given, to find its root.

Let this root be $$x$$, and we have the equation
$$\dfrac{3x^2-x}{2}=a$$, or $$3x^2-x=2a$$, or
$$x^2=\frac{1}{3}x+\frac{2a}{3}$$; by means of
which we find $$x=\frac{1}{6}+\surd\left(\frac{1}{36}+\frac{2a}{3}\right)$$,
that is,

$$x=\dfrac{1+\surd(24a+1)}{6}.$$

Therefore, when $$a$$ is a real pentagon, $$24a+1$$ must be a square.

Let 330, for example, be the given pentagon, the root will be

$$x=\dfrac{1+\surd(7921)}{6} = \dfrac{1+89}{6}=15.$$

<span class="art">665</span> Again, let $$a$$ be a given hexagonal number, the root of which is required.

If we suppose it $$=x$$, we shall have $$2x^2-x=a$$, or $$x^2=\frac{1}{2}x+\frac{1}{2}a$$;
and this gives

$$x=\frac{1}{4}+\surd\left(\frac{1}{16}+\frac{1}{2}a\right) = \dfrac{1+\surd(8a+1)}{4}.$$

So that, in order that $$a$$ may be really a hexagon, $$8a + 1$$
must become a square; whence we see, that all hexagonal
numbers are contained in triangular numbers; but it is not
the same with the roots.

For example, let the hexagonal number be 1225, its root will be

$$x=\dfrac{1+\surd 9801}{4} = \dfrac{1+99}{4}=25.$$

<span class="art">666</span> Suppose $$a$$ an heptagonal number, of which the root is required.

Let this root be $$x$$, then we shall have $$\dfrac{5x^2-3x}{2}=a$$, or
$$x^2=\frac{3}{5}x+\frac{2}{5}a$$, which gives

$$x=\frac{3}{10}+\surd\left(\frac{9}{100}+\frac{2}{3}a\right)=\dfrac{3+\surd(40a+9)}{10};$$

therefore the heptagonal numbers have this property, that if
they be multiplied by 40, and 9 be added to the product,
the sum will always be a square.

Let the heptagon, for example, be 2059; its root will be found

$$=x=\dfrac{3+\surd(82369)}{10} = \dfrac{3+287}{10} = 29.$$

Let the heptagon, for example, be 2059; its root will be found

$$=x=\dfrac{3+\surd(82369)}{10} = \dfrac{3+287}{10} = 29.$$

<span class="art">667</span> Let us suppose a an octagonal number, of which
the root $$x$$ is required.

We shall here have $$3x^2-2x=a$$, or $$x^2=\frac{2}{2}x+\frac{1}{3}a$$,
whence results

$$x=\frac{1}{3}+\surd\left(\frac{1}{9}+\frac{1}{3}a\right) = \dfrac{1+\surd(3a+1)}{3}.$$

Consequently, all octagonal numbers are such, that if multiplied by 3, and unity be added to the product,
the sum is consequently a square.

For example, let 3816 be an octagon; its root will be

$$x=\dfrac{1+\surd 11449}{3} = \dfrac{1+107}{3} = 36.$$

<span class="art">668</span> Lastly, let $$a$$ be a given $$n$$-gonal number, the root of
which it is required to assign; we shall then, by the last
formula, have this equation:

$$\dfrac{(n-2)x^2-(n-4)x}{2} = a,$$

or $$(n-2)x^2-(n-4)x=2a$$; consequently,

$$x^2=\dfrac{(n-4)x}{n-2}+\dfrac{2a}{n-2};$$

whence,

$$x=\dfrac{n-4}{2(n-2)} + \surd \left( \dfrac{(n-4)^2}{4(n-2)^2}+\dfrac{2a}{n-2}\right),$$

or

$$x=\dfrac{n-4}{2(n-2)} + \surd \left( \dfrac{(n-4)^2}{4(n-2)^2}+\dfrac{8(n-2)a}{4(n-2)^2}\right),$$

or

$$x=\dfrac{n-4+\surd(8(n-2)a+(n-4)^2)}{2(n-2)}.$$

This formula contains a general rule for finding all the
possible polygonal roots of given numbers.

For example, let there be given the 24-gonal number, 3009:
since $$a$$ is here = 3009 and $$n=24$$, we have
$$n-2=22$$ and $$n-4=20$$; wherefore the root

$$x=\dfrac{20+\surd(529584+400)}{44} = \dfrac{20+728}{44} = 17.$$

#### Editions

1. Leonhard Euler. *Elements of Algebra*. Translated by Rev. John Hewlett. Third Edition. Longmans, Hurst, Rees, Orme, and Co. London. 1822.
    - [Part {{ page.part }}. Section {{ page.section }}. {{ page.title }}](/assets/euler/en/IV-7.pdf)
2. Leonhard Euler. *Vollständige Anleitung zur Algebra. Mit den Zusätzen von Joseph Louis Lagrange.* Herausgegeben von Heinrich Weber. B. G. Teubner. Leipzig and Berlin. 1911. Leonhardi Euleri Opera omnia. Series prima. Opera mathematica. Volumen primum.
    - [Zweyter Theil. Erster Abschnitt. Capitel 7. Von der Ausziehung der Wurzeln aus den vieleckigten Zahlen](/assets/euler/de/II-I-7.pdf)