---
layout: page
title: Chapter 4. "Of the Resolution of two or more Equations of the First Degree."
part: I
section: IV
chapter: 4
---

### Part {{ page.part }}. Section {{ page.section }}. {{ page.title }}

<span class="art">605</span> It frequently happens that we are obliged to introduce into algebraic calculations
two or more unknown quantities, represented by the letters $$x$$, $$y$$, $$z$$: and if the question
is determinate, we are brought to the same number of equations as there are unknown quantities;
from which it is then required to deduce those quantities. As we consider, at present, those
equations only, which contain no powers of an unknown quantity higher than the first, and no
products of two or more unknown quantities, it is evident that all those equations have the
form $$az+by+cx=d$$.

<span class="art">606</span> Beginning therefore with two equations, we shall
endeavour to find from them the value of $$x$$ and $$y$$: and, in
order that we may consider this case in a general manner, let
the two equations be,

$$\textrm{I) } \; ax + by = c; \quad \textrm{and} \quad \textrm{II) } \; fx + gy = h;$$

in which, $$a$$, $$b$$, $$c$$, and $$f$$, $$g$$, $$h$$, are known numbers. It is
required, therefore, to obtain, from these two equations, the
two unknown quantities $$x$$ and $$y$$.

<span class="art">607</span> The most natural method of proceeding will readily
present itself to the mind; which is, to determine, from both
equations, the value of one of the unknown quantities, as for
example $$x$$, and to consider the equality of those two values;
for then we shall have an equation, in which the unknown
quantity $$y$$ will be found by itself, and may be determined
by the rules already given. Then, knowing $$y$$, we shall have
only to substitute its value in one of the quantities that
express $$x$$.

<span class="art">608</span> According to this rule, wo obtain from the first
equation, $$x=\dfrac{c-by}{a}$$, and from the second, $$x=\dfrac{h-gy}{f}$$:
then putting these vaues equal to each other, we have this
new equation:

$$\dfrac{c-by}{a}=\dfrac{h-gy}{f};$$

multiplying by $$a$$, the product is

$$c-by=\dfrac{ah-agy}{f};$$

and then by $$f$$, the product is

$$fc-fby = ah-agy;$$

adding $$agy$$, we have

$$fc-fby+agy = ah;$$

subtracting $$fc$$, gives

$$-fby+agy = ah-fc;$$

or

$$(ag-bf)y = ah-fc;$$

lastly, dividing by $$ag-bf$$, we have

$$y = \dfrac{ah-fc}{ag-bf}.$$

In order now to substitute this value of $$y$$ in one of the
two values which we have found of $$x$$, as in the first, where
$$x=\dfrac{c-by}{a}$$, we shall first have

$$-by = - \dfrac{abh-bcf}{ag-bf};$$

whence

$$c-by= c- \dfrac{abh-bcf}{ag-bf}=\dfrac{acg-bcf-abh+bcf}{ag-bf}=\dfrac{acg-abh}{ag-bf};$$

and dividing by $$a$$,

$$x = \dfrac{c-by}{a} = \dfrac{cg-bh}{ag-bf}.$$

<span class="art">609</span> *Question 1.* To illustrate this method by examples,
let it be proposed to find two numbers, whose sum may be
15, and difference 7.

Let us call the greater number $$x$$, and the less $$y$$: then we shall have

$$\textrm{I) } \; x + y = 15, \quad \textrm{and} \quad \textrm{II) } \; x - y =7.$$

The first equation gives $$x = 15 - y$$ and the second, $$x = 7 + y$$;
whence results this equation, $$15-y = 7 + y$$. So that
$$15 = 7 + 2y$$; $$2y = 8$$, and $$y=4$$; by which means we find $$x = 11$$.

So that the less number is 4, and the greater is 11.

<span class="art">610</span> *Question 2.* We may also generalise the preceding
question, by requiring two numbers, whose sum may be $$a$$,
and the difference $$b$$.

Let the greater of the two numbers be expressed by $$x$$, and
the less by $$y$$; we shall then have

$$\textrm{I) } \; x+y=a,\quad \textrm{and} \quad \textrm{II) } \; x-y=b.$$

Here the first equation gives $$x = a - y$$, and the second $$x = b + y$$. Therefore,
$$a-y=b+y$$; $$a=b+2y$$; $$2y=a-b$$; lastly,

$$y=\dfrac{a-b}{2},$$

and, consequently,

$$x=a-y = a-\dfrac{a-b}{2}=\dfrac{a+b}{2}.$$

Thus, we find the greater number, or $$x$$, is $$\dfrac{a+b}{2}$$,
and the less, or $$y$$, is $$\dfrac{a-b}{2}$$; or, which comes to the same,

$$x= \frac{1}{2}a+\frac{1}{2}b, \quad \textrm{and} \quad y=\frac{1}{2}a-\frac{1}{2}b.$$

Hence we derive the following
theorem: When the sum of any two numbers is $$a$$, and their
difference is $$b$$, the greater of the two numbers will be equal
to half the sum *plus* half the difference; and the less of the
two numbers will be equal to half the sum *minus* half the
difference.

<span class="art">611</span> We may resolve the same question in the following manner: Since the two equations are,

$$x+y=a, \quad \textrm{and} \quad x-y=b,$$

if we add the one to the other, we have

$$2x=a+b.$$

Therefore $$x=\dfrac{a+b}{2}$$.

Lastly, subtracting the same equations from each other,
we have

$$2y=a-b;$$

and therefore

$$y=\dfrac{a-b}{2}.$$

<span class="art">612</span> *Question 3.* A mule and an ass were carrying
burdens amounting to several hundred weight. The ass
complained of his, and said to the mule, I need only one
hundred weight of your load, to make mine twice as heavy
as yours; to which the mule answered, But if you give
me a hundred weight of yours, I shall be loaded three times
as much you will be. How many hundred weight did each
carry?

Suppose the mule's load to be $$x$$ hundred weight, and that
of the ass to be $$y$$ hundred weight. If the mule gives one
hundred weight to the ass, the one will have $$y + 1$$, and there
will remain for the other $$x - 1$$; and since, in this case,
the ass is loaded twice as much as the mule, we have $$y + 1 = 2x - 2$$.

Farther, if the ass gives a hundred weight to the mule,
the latter has $$x + 1$$, and the ass retains $$y - 1$$; but the
burden of the former being now three times that of the
latter, we have $$x + 1 = 3y - 3$$.

Consequently our two equations will be,

$$\textrm{I) } \; y + 1 = 2x-2, \quad \textrm{and} \quad \textrm{II) } \; x+1=3y-3.$$

From the first, $$x=\dfrac{y+3}{2}$$, and the second gives
$$x = 3y-4$$; whence we have the new equation $$\dfrac{y+3}{2}=3y-4$$,
which gives $$y=\dfrac{11}{5}$$; this also determines the value
of $$x$$, which becomes $$2\frac{3}{5}$$.

The mule therefore carried $$2\frac{3}{5}$$ hundred weight,
and the ass $$2 \frac{1}{5}$$ hundred weight.

<span class="art">613</span> When there are three unknown numbers, and as
many equations; as, for example,

$$
\begin{gather}
\textrm{I)} \; x+y-z=8\\
\textrm{II)} \; x+z-y=9\\
\textrm{III)} \; y+z-x=10;
\end{gather}
$$

we begin, as before, by deducing a value of $$x$$ from each,
and have,

$$
\begin{gather}
\textrm{I)} \; x=8+z-y\\
\textrm{II)} \; x=9+y-z\\
\textrm{III)} \; x=y+z-10.
\end{gather}
$$

Comparing the first of these values with the second,
and after that with the third, we have the following
equations:

$$
\begin{gather}
\textrm{I)} \; 8+z-y=9+y-z,\\
\textrm{II)} \; 8+z-y=y+z-10.
\end{gather}
$$

Now, the first gives $$2z-2y = 1$$, and, by the second,
$$2y=18$$, or $$y = 9$$; if therefore we substitute this value of
$$y$$ in $$2z-2y = 1$$, we have $$2z- 18 = 1$$, or $$2z = 19$$, so
that $$z=9\frac{1}{2}$$; it remains, therefore, only to determine $$x$$,
which is easily found $$=8\frac{1}{2}$$.

Here it happens, that the letter $$z$$ vanishes in the last
equation, and that the value of $$y$$ is found immediately;
but if this had not been the case, we should have had
two equations between $$z$$ and $$y$$, to be resolved by the preceding rule.

<span class="art">614</span> Suppose we had found the three following equations:

$$
\begin{gather}
\textrm{I)} \; 3x+5y-4z=25,\\
\textrm{II)} \; 5x-2y+3z=46,\\
\textrm{III)} \; 3y+5z-x=62.
\end{gather}
$$

If we deduce from each the value of $$x$$ we shall have

$$
\begin{gather}
\textrm{I)} \; x=\dfrac{25-5y+4z}{3},\\
\textrm{II)} \; x=\dfrac{46+2y-3z}{5},\\
\textrm{III)} \; x=3y+5z-62.
\end{gather}
$$

Comparing these three values together, and first the third
with the first, we have

$$3y+5z-62=\dfrac{25-5y+4z}{3};$$

multiplying bv 3, gives

$$9y+15z-186=25-5y+4z;$$

so that $$9y + 15z = 211 - 5y - 4z$$, and

$$14y+11z=211.$$

Comparing also the third with the second, we have

$$3y+5z-62=\dfrac{46+2y-3z}{5},$$

or $$46+2y-3z=15y+25z-310$$,
which, when reduced, becomes

$$356=13y+28z.$$

We shall now deduce, from these two new equations, the value of $$y$$:

$$\textrm{I)} \; 14y+11z=211; \quad \textrm{or} \quad 14y=211-11z,$$

and $$y = \dfrac{211-11z}{14}$$.

$$\textrm{II)} \; 13y+28z=356; \quad \textrm{or} \quad 13y=356-28z,$$

and $$y = \dfrac{356-28z}{13}$$.

These two values form the new equation

$$\dfrac{211-11z}{14}=\dfrac{356-28z}{13},$$

whence $$2743-143z=4984-392z$$, or $$249z=2241$$, and $$z=9$$.

This value being substituted in one of the two equations
of $$y$$ and $$z$$, we find $$y=8$$; and, lastly, a similar substitution
in one of the three values of $$x$$, will give $$x=7$$.

<span class="art">615</span> If there were more than three unknown quantities to
determine, and as many equations to resolve, we should proceed in the same manner;
but the calculations would often
prove very tedious.

It is proper, therefore, to remark, that, in each particular
case, means may always be discovered of greatly facilitating
the solution; which consist in introducing into the calculation, beside
the principal unknown quantities, a new
unknown quantity arbitrarily assumed, such as, for example,
the sum of all the rest; and when a person is a little accustomed to such
calculations, he easily perceives what is
most proper to be done. The following examples may
serve to facilitate the application of these artifices.

<span class="art">616</span> *Question 4.* Three persons, A, B, and C, play together; and, in the first game,
a loses to each of the other two, as much money as each of them has. In the next
game, B loses to each of the other two, as much money as
they then had. Lastly, in the third game, A and B gain
each, from C, as much money as they had before. On
leaving off, they find that each has an equal sum, namely,
24 guineas. Required, with how much money each sat
down to play?

Suppose that the stake of the first person was $$x$$, that of
the second $$y$$, and that of the third $$z$$: also, let us make the
sum of all the stakes, or $$x + y + z$$, $$= s$$. Now, A losing in
the first game as much money as the other two have, he
loses $$s - x$$ (for he himself having had $$x$$, the two others
must have had $$s - x$$); therefore there will remain to him
$$2x-s$$; also B will have $$2y$$, and C will have $$2z$$.

So that, after the first game, each will have as follows:
$$A = 2x - s$$, $$B = 2y$$, and $$C = 2z$$.

In the second game, B, who has now $$2y$$, loses as much
money as the other two have, that is to say, $$s - 2y$$; so that
he has left $$4y - s$$. With regard to the other two, they
will each have double what they had; so that after the
second game, the three persons have as follows: $$A = 4x - 2s$$,
$$B = 4y-s$$, and $$C = 4z$$.

In the third game, C, who has now $$4z$$, is the loser; he
loses to A, $$4x - 2s$$, and to B, $$4y-s$$; consequently, after
this game, they will have:

$$A=8x-4s,\quad B=8y-2s,\; \textrm{and} \; c=8z-s.$$

Now, each having at the end of this game 24 guineas, we
have three equations, the first of which immediately gives $$x$$,
the second $$y$$, and the third $$z$$; farther, $$s$$ is known to be 72,
since the three persons have in all 72 guineas at the end of
the last game; but it is not necessary to attend to this at
first; since we have,

$$
\begin{gather}
\textrm{I)} \; 8x-4s=24, \; \textrm{or} \; 8x=24+4s, \; \textrm{or} \; x=3+\frac{1}{2}s;\\
\textrm{II)} \; 8y-2s=24, \; \textrm{or} \; 8y=24+2s, \; \textrm{or} \; y=3+\frac{1}{4}s;\\
\textrm{III)} \; 8z-s=24, \; \textrm{or} \; 8z=24+s, \; \textrm{or} \; z=3+\frac{1}{8}s;
\end{gather}
$$

and adding these three values, we have $$x+y+z=9+\frac{7}{8}s$$.
So that, since $$x+y+z=s$$, we have $$s=9+\frac{7}{8}s$$;
and, consequently, $$\frac{1}{8}s=9$$, and $$s=72$$.

If we now substitute this value of $$s$$ in the expressions
which we have found for $$x$$, $$y$$, and $$z$$, we shall find that,
before they began to play, A had 39 guineas, B 21, and
C 12.

This solution shows, that, by means of an expression for
the sum of the three unknown quantities, we may overcome
the difficulties which occur in the ordinary method.

<span class="art">617</span> Although the preceding question appears difficult at
first, it may be resolved even without algebra, by proceeding
inversely. For since the players, when they left off, had
each 24 guineas, and, in the third game, A and B doubled
their money, they must have had before that last game, as
follows:

$$A = 12, \quad B = 12, \quad \textrm{and} \quad C = 48.$$

In the second game, A and C doubled their money; so
that before that game they had;

$$A = 6, \quad B = 42, \quad \textrm{and} \quad C=24.$$

Lastly, in the first game, A and C gained each as much
money as they began with; so that at first the three persons
had:

$$A=39, \quad B=21, \quad C=12.$$

The same result as we obtained by the former solution.

<span class="art">618</span> *Question 5.* Two persons owe conjointly 29 pistoles; they have both money,
but neither of them enough to enable him, singly, to discharge this common debt: the
first debtor says therefore to the second, If you give me ⅔ of
your money, I can immediately pay the debt; and the
second answers, that he also could discharge the debt, if the
other would give him ¾ of his money. Required, how many
pistoles each had?

Suppose that the first has $$x$$ pistoles, and that the second
has $$y$$ pistoles.

Then we shall first have, $$x+\frac{2}{3}y=29$$;
and also, $$y+\frac{3}{4}x=29$$.

The first equation gives $$x=29-\frac{2}{3}y$$,
and the second $$x=\frac{116-4y}{3}$$;
so that $$29-\frac{2}{3}y=\frac{116-4y}{3}$$.

From which equation, we obtain $$y=14\frac{1}{2}$$;
Therefore $$x=19\frac{1}{3}$$.

Hence the first person had $$19\frac{1}{3}$$ pistoles, and the second
had $$14\frac{1}{2}$$ pistoles.

<span class="art">619</span> *Question 6.* Three brothers bought a vineyard for
a hundred guineas. The youngest says, that he could pay
for it alone, if the second gave him half the money which he
had; the second says, that if the eldest would give him only
the third of his money, he could pay for the vineyard singly;
lastly, the eldest asks only a fourth part of the money of
the youngest, to pay for the vineyard himself. How much
money had each?

Suppose the first had $$x$$ guineas; the second, $$y$$ guineas;
the third, $$z$$ guineas; we shall then have the three following
equations:

$$
\begin{gather}
\textrm{I)} \; x+\frac{1}{2}y=100;\\
\textrm{II)} \; y+\frac{1}{3}z=100;\\
\textrm{III)} \; z+\frac{1}{4}x=100;
\end{gather}
$$

two of which only give the value of $$x$$, namely,

$$
\begin{gather}
\textrm{I)} \; x=100-\frac{1}{2}y,\\
\textrm{III)} \; x=400-4z.
\end{gather}
$$

So that we have the equation,
$$100-\frac{1}{2}y=400-4z$$, or $$4z-\frac{1}{2}y=300$$, which must
be combined with the second, in order to determine $$y$$ and $$z$$.
Now, the second equation was, $$y+\frac{1}{3}z=100$$: we
therefore deduce from it $$y=100-\frac{1}{3}z$$; and the equation
found last being $$4z-\frac{1}{2}y=300$$, we have $$y=8z-600$$.
The final equation, therefore, becomes
$$100-\frac{1}{3}z=8z-600$$; so that $$8\frac{1}{3}z=700$$, or $$\frac{25}{3}z=700$$, and
$$z=84$$. Consequently,
$$y=100-28=72$$, and $$x=64$$.

The youngest therefore had 64 guineas, the second had 72
guineas, and the eldest had 84 guineas.

<span class="art">620</span> As, in this example, each equation contains only two
unknown quantities, we may obtain the solution required in
an easier way.

The first equation gives $$y = 200 - 2x$$, so that $$y$$ is determined by $$x$$; and if we 
substitute this value in the second equation, we have
$$200-2x+\frac{1}{3}z=100$$; therefore $$\frac{1}{3}z=2x-100$$, and $$z=6x-300$$.

So that $$z$$ is also determined by $$x$$; and if we introduce this value into
the third equation, we obtain $$6x-300+\frac{1}{4}x=100$$, in which $$x$$ stands alone,
and which, when reduced to $$25x-1600=0$$, gives $$x=64$$. Consequently,
$$y=200-128=72$$, and $$z=384-300=84$$.

<span class="art">621</span> We may follow the same method, when we have a
greater number of equations. Suppose, for example, that
we have in general;

$$
\begin{gather}
\textrm{I)} \; u+\dfrac{x}{a}=n,\\
\textrm{II)} \; x+\dfrac{y}{b}=n,\\
\textrm{III)} \; y+\dfrac{z}{c}=n,\\
\textrm{IV)} \; z+\dfrac{u}{d}=n;
\end{gather}
$$

or, destroying the fractions, these equations become,

$$
\begin{gather}
\textrm{I)} \; au+x=an,\\
\textrm{II)} \; bx+y=nb,\\
\textrm{III)} \; cy+z=nc,\\
\textrm{IV)} \; dz+u=nd;
\end{gather}
$$

Here, the first gives immediately $$x = an-au$$, and, this
value being substituted in the second, we have $$abn-abu+y=bn$$;
so that $$y =bn-abn+abu$$; and the substitution of this value, in the third equation, gives
$$bcn-abcn+abcu+z=cn$$; therefore

$$z=cn-bcn+abcn-abcu.$$

Substituting this in the fourth equation, we have

$$cdn-bcdn+abcdn-abcdu+u=dn.$$

So that

$$dn-cdn+bcdn-abcdn=abcdu-u,$$

or

$$(abcd-1)\cdot u = abcdn-bcdn+cdn-dn;$$

whence we have

$$u = \dfrac{abcdn-bcdn+cdn-dn}{abcd-1}=\dfrac{n\cdot (abcd-bcd+cd-d)}{abcd-1}.$$

And, consequently, by substituting this value of $$u$$ in the
equation, $$x = an - au$$, we have

$$
\begin{gather}
x=\dfrac{abcdn-acdn+adn-an}{abcd-1} = \dfrac{n\cdot (abcd-acd+ad-a)}{abcd-1},\\
y=\dfrac{abcdn-abdn+abn-bn}{abcd-1} = \dfrac{n\cdot (abcd-abd+ab-b)}{abcd-1},\\
z=\dfrac{abcdn-abcn+bcn-cn}{abcd-1} = \dfrac{n\cdot (abcd-abc+bc-c)}{abcd-1},\\
u=\dfrac{abcdn-bcdn+cdn-dn}{abcd-1} = \dfrac{n\cdot (abcd-bcd+cd-d)}{abcd-1}.
\end{gather}
$$

<span class="art">622</span> *Question 7.* A captain has three companies, one of
Swiss, another of Swabians, and a third of Saxons. He
wishes to storm with part of these troops, and he promises a
reward of 901 crowns, on the following condition; namely,
that each soldier of the company, which assaults, shall receive 1 crown,
and that the rest of the money shall be equally
distributed among the two other companies. Now, it is
found, that if the Swiss make the assault, each soldier of the
other companies will receive half-a-crown; that, if the Swabians assault,
each of the others will receive ⅓ of a crown;
and, lastly, if the Saxons make the assault, each of the others
will receive ¼ of a crown. Required the number of men in
each company?

Let us suppose the number of Swiss to be $$x$$, that of
Swabians $$y$$, and that of Saxons $$z$$. And let us also make
$$x+y+z= s$$, because it is easy to see, that, by this, we
abridge the calculation considerably. If, therefore, the Swiss
make the assault, their number being $$x$$, that of the other
will be $$s - x$$: now, the former receive 1 crown, and the
latter half-a-crown; so that we shall have,

$$x+\frac{1}{2}s-\frac{1}{2}x=901.$$

In the same manner, if the Swabians make the assault, we have

$$y+\frac{1}{3}s-\frac{1}{3}y=901.$$

And lastly, if the Saxons make the assault, we have,

$$z+\frac{1}{4}s-\frac{1}{4}z=901.$$

Each of these three equations will enable us to determine
one of the unknown quantities, $$x$$, $$y$$, and $$z$$;

$$
\begin{gather}
x=1802-s,\\
2y=2703-s,\\
3z=3604-s.
\end{gather}
$$

And if we now take the values of $$6x$$, $$6y$$, and $$6z$$, and
write those values one above the other, we shall have

$$
\begin{gather}
6x=10812-6s,\\
6y=8109-3s,\\
6z=7208-2s,
\end{gather}
$$

and, by addition, $$6s=26129-11s$$; or $$17s=26129$$; so that
$$s=1537$$; which is the whole number of soldiers.
By this means we find,

$$
\begin{gather}
x=1802-1537=265;\\
2y=2703-1537=1166, \; \textrm{or } \; y=583;\\
3x=3604-1537=2067, \; \textrm{or } \; z=689.
\end{gather}
$$

The company of Swiss therefore has 265 men; that of
Swabians 583; and that of Saxons 689.
    

#### Editions

1. Leonhard Euler. *Elements of Algebra*. Translated by Rev. John Hewlett. Third Edition. Longmans, Hurst, Rees, Orme, and Co. London. 1822.
    - [Part {{ page.part }}. Section {{ page.section }}. {{ page.title }}](/EulerAlgebra/en/IV-4.pdf)
2. Leonhard Euler. *Vollständige Anleitung zur Algebra. Mit den Zusätzen von Joseph Louis Lagrange.* Herausgegeben von Heinrich Weber. B. G. Teubner. Leipzig and Berlin. 1911. Leonhardi Euleri Opera omnia. Series prima. Opera mathematica. Volumen primum.
    - [Zweyter Theil. Erster Abschnitt. Capitel 4. Von Auflösung zweyer oder mehr Gleichungen vom ersten Grad](/EulerAlgebra/de/II-I-4.pdf)