---
layout: page
title: Chapter 2. "Of the Resolution of Simple Equations, or Equations of the First Degree."
part: I
section: IV
chapter: 1
---

### Part {{ page.part }}. Section {{ page.section }}. {{ page.title }}

<span class="art">573</span> When the number sought, or the unknown quantity,
is represented by the letter $$x$$, and the equation we have
obtained is such, that one side contains only that $$x$$, and the
other simply a known number, as, for example, $$x=25$$, the
value of $$x$$ is already known. We must always endeavour,
therefore, to arrive at such a form, however complicated
the equation may be when first obtained: and, in the
course of this section, the rules shall be given, and
explained, which serve to facilitate these reductions.

<span class="art">574</span> Let us begin with the simplest cases, and suppose,
first, that we have arrived at the equation $$x + 9 = 16$$.
Here we see immediately that $$x=7$$: and, in general, if
we have found $$x + a = b$$, where $$a$$ and $$b$$ express any
known numbers, we have only to subtract $$a$$ from both
sides, to obtain the equation $$x=b-a$$, which indicates the
value of $$x$$. 

<span class="art">575</span> If we have the equation $$x-a=b$$, we must add
$$a$$ to both sides, and shall obtain the value of $$x=b +a$$.
We must proceed in the same manner, if the equation
have this form, $$x-a=a^2+1$$: for we shall immediately
find $$x=a^2 +a+ 1$$.

In the equation $$x-8a=20-6a$$, we find
$$x=20-6a+8a$$, or $$x=20+2a$$.

And in this, $$x+6a=20+3a$$, we have
$$x=20+3a-6a$$, or $$x=20-3a$$. 

<span class="art">576</span> If the original equation have this form, $$x - a +b=c$$,
we may begin by adding $$a$$ to both sides, which will
give $$x + b =c + a$$; and then subtracting $$b$$ from both
sides, we shall find $$x = c +a - b$$. But we might also
add $$+ a - b$$ at once to both sides; and thus obtain
immediately $$x=c+a-b$$.

So likewise in the following examples:  
If $$x-2a+3b=0$$, we have $$x=2a-3b$$.  
If $$x-3a+2b=25+a+2b$$, we have $$x=25+4a$$.  
If $$x-9 +6a=25+2a$$, we have $$x=34-4a$$.

<span class="art">577</span> When the given equation has the form $$ax=b$$, we
only divide the two sides by $$a$$, to obtain $$x = \dfrac{b}{a}$$. But if the
equation have the form $$ax+b-c=d$$, we must first make
the terms that accompany $$ax$$ vanish, by adding to both
sides $$- b + c$$; and then, dividing the new equation $$ax=d-b+c$$
by $$a$$, we shall have $$x = \dfrac{d-b+c}{a}$$.

The same value of $$x$$ would have been found by
subtracting $$+ b -c$$ from the given equation: that is, we
should have had, in the same form,

$$ax = d - b + c, \quad \textrm{and} \quad x = \dfrac{d-b+c}{a}.$$

Hence,  
If $$2x+5=17$$, we have $$2x=12$$, and $$x=6$$.  
If $$3x-8=7$$, we have $$3x= 15$$, and $$x=5$$.  
If $$4x - 5 - 3a = 15 + 9a$$, we have $$4x = 20 + 12a$$,
and consequently $$x=5 + 3a$$.

<span class="art">578</span> When the first equation has the form $$\dfrac{x}{a}=b$$, we
multiply both sides by $$a$$, in order to have $$x = ab$$.

But if it is $$\dfrac{x}{a} + b - c = d$$, we must first make
$$\dfrac{x}{a} =  d- b + c$$; after which we find

$$x=(d -b + c)a=ad-ab + ac.$$

Let $$\frac{1}{2}x-3=4$$, then $$\frac{1}{2}x=7$$, and $$x= 14$$.  
Let $$\frac{1}{3}x - 1 + 2a = 3 + a$$, then $$\frac{1}{3}x = 4 - a$$, and
$$x=12-3a$$.  
Let $$\dfrac{x}{a-1}-1=a$$, then $$\dfrac{x}{a-1} =a + 1$$, and $$x = a^2 - 1$$.

<span class="art">579</span> When we have arrived· at such an equation as 
$$\dfrac{ax}{b} = c$$, we first multiply by $$b$$, in order to have $$ax =bc$$,
and then dividing by $$a$$, we find $$x = \dfrac{bc}{a}$$.

If $$\dfrac{ax}{b}- c =d$$, we begin by giving the equation this
form, $$\dfrac{ax}{b} = d + c$$; after which, we obtain the value of
$$ax = bd + bc$$, and then that of $$x = \dfrac{bd+bc}{a}$$.

Let $$\frac{2}{3}x - 4 = 1$$, then $$\frac{2}{3}x = 5$$, and $$2x = 15$$; whence
$$x=\frac{15}{2}=7\frac{1}{2}$$.

If $$\frac{3}{4}x+\frac{1}{2}=5$$, we have $$\frac{3}{4}x =5 -\frac{1}{2} =\frac{9}{2}$$; whence
$$3x=18$$, and $$x=6$$.

<span class="art">580</span> Let us now consider a case, which may frequently
occur; that is, when two or more terms contain the letter
$$x$$, either on one side of the equation, or on both.

If those terms are all on the same side, as in the equation $$x+\frac{1}{2}x+5=11$$,
we have $$x+\frac{1}{2}x=6$$; or $$3x=12$$; and
lastly, $$x=4$$.

Let $$x + \frac{1}{2}x + \frac{1}{3}x = 44$$, be an equation, in which the
value of $$x$$ is required. If we first multiply by 3, we have
$$4x + \frac{3}{2}x = 132$$; then multiplying by 2, we have $$11x =264$$;
wherefore $$x=24$$. We might have proceeded in a
more concise manner, by beginning with the reduction of
the three terms which contain $$x$$ to the single term $$\frac{11}{6}x$$;
and then dividing the equation $$\frac{11}{6}x=44$$ by 11. This
would have given $$\frac{1}{6}x=4$$, and $$x=24$$, as before.

Let $$\frac{2}{3}x - \frac{3}{4}x + \frac{1}{2}x =1$$. We shall have, by reduction,
$$\frac{5}{12}x=1$$, or $$5x=12$$, and $$x=2\frac{2}{5}$$.

And, generally, let $$ax - bx + cx = d$$; which is the
same as $$(a-b+c)x=d$$, and, by division, we derive $$x=\dfrac{d}{a-b+c}$$.

<span class="art">581</span> When there are terms containing $$x$$ on both sides
of the equation, we begin by making such terms vanish
from that side from which it is most easily expunged; that
is to say, in which there are the fewest terms so involved.

If we have, for example, the equation $$3x+2=x+ 10$$,
we must first subtract $$x$$ from both sides, which gives
$$2x+2= 10$$; wherefore $$2x=8$$, and $$x=4$$. 

Let $$x + 4 = 20 - x$$; here it is evident that
$$2x + 4 = 20$$; and consequently $$2x= 16$$, and $$x=8$$.

Let $$x+8=32-3x$$, this gives us $$4x+8=32$$; or $$4x=24$$,
whence $$x=6$$.

Let $$15-x=20-2x$$, here we shall have
$$15 +x=20$$, and $$x=5$$.

Let $$1 +x=5-\frac{1}{2}x$$; this becomes $$1 +\frac{3}{2}x=5$$, or $$\frac{3}{2}x=4$$;
therefore $$3x=8$$; and lastly, $$x=\dfrac{8}{3}=2\frac{2}{3}$$.

If $$\frac{1}{2}-\frac{1}{3}x=\frac{1}{3}-\frac{1}{4}x$$,
we must add $$\frac{1}{3}x$$, which gives $$\frac{1}{2}=\frac{1}{3} +\frac{1}{12}x$$;
subtracting $$\frac{1}{3}$$, and transposing the terms, there
remains $$\frac{1}{12}x=\frac{1}{6}$$; then multiplying by 12, we obtain $$x=2$$.

If $$1\frac{1}{2}-\frac{2}{3}x=\frac{1}{4}+\frac{1}{2}x$$, we add $$\frac{2}{3}x$$, which gives
$$1\frac{1}{2}=\frac{1}{4}+\frac{7}{6}x$$;
then subtracting $$\frac{1}{4}$$, and transposing, we have $$\frac{7}{6}x= 1\frac{1}{4}$$,
whence, by multiplying by 6 and dividing by 7, we deduce $$x=1\frac{1}{14}=\frac{15}{14}$$.

<span class="art">582</span> If we have an equation in which the unknown
number $$x$$ is a denominator, we must make the fraction vanish
by multiplying the whole equation by that denominator.

Suppose that we have found $$\frac{100}{x} -8= 12$$, then, adding
8, we have $$\frac{100}{x} = 20$$; and multiplying by $$x$$, it becomes
$$100=20x$$; lastly, dividing by 20, we find $$x=5$$.

Let now $$\dfrac{5x+3}{x-1} = 7$$; here, multiplying by $$x -1$$,
we $$5x+3=7x-7$$; and subtracting $$5x$$, there remains
$$3 =2x-7$$; then adding 7, we have $$2x= 10$$; whence
$$x=5$$.

<span class="art">583</span> Sometimes, also, radical signs are found in equations
of the first degree. For example: A number $$x$$, below 100,
is required, such, that the square root of $$100-x$$ may be
equal to 8; or $$\surd(100-x)=8$$. The square of both sides
will give $$100-x=64$$, and adding $$x$$, we have $$100=64+x$$:
whence we obtain $$x=100-64=36$$.

Or, since $$100-x=64$$, we might have subtracted 100
from both sides: which would have given $$-x= -36$$; or,
multiplying by $$-1$$, $$x=36$$.

<span class="art">584</span> Lastly, the unknown number $$x$$ is sometimes found
as an exponent, of which we have already seen some
examples; and, in this case, we must have recourse to
logarithms. 

Thus, when we have $$2^x=512$$, we take the logarithms of
both sides; whence we obtain $$x \log 2 = \log 512$$; and
dividing by $$\log 2$$, we find $$x = \dfrac{\log 512}{\log 2}$$. The Tables then give,

$$x = \dfrac{2.7092700}{0.3010300} = \dfrac{27092700}{3010300},$$

or $$x=9$$.

Let $$5 \cdot 3^{2x} - 100 = 305$$;  we add 100, which gives
$$5 \cdot 3^{2x} = 405$$; dividing by 5, we have $$3^{2x}= 81$$; and taking
the logarithms,
$$2x \log 3=\log 81$$,
and dividing by $$2 \log 3$$,
we have

$$x = \dfrac{\log 81}{2 \log 3},$$

or,

$$x = \dfrac{\log 81}{\log 9};$$

whence

$$x = \dfrac{1.9084850}{0.9542425}=\dfrac{19084850}{09542425}=2.$$

#### Editions

1. Leonhard Euler. *Elements of Algebra*. Translated by Rev. John Hewlett. Third Edition. Longmans, Hurst, Rees, Orme, and Co. London. 1822.
    - [Part {{ page.part }}. Section {{ page.section }}. {{ page.title }}](/assets/euler/en/IV-2.pdf)
2. Leonhard Euler. *Vollständige Anleitung zur Algebra. Mit den Zusätzen von Joseph Louis Lagrange.* Herausgegeben von Heinrich Weber. B. G. Teubner. Leipzig and Berlin. 1911. Leonhardi Euleri Opera omnia. Series prima. Opera mathematica. Volumen primum.
    - [Zweyter Theil. Erster Abschnitt. Capitel 2. Von den Gleichungen des ersten Grads und ihrer Auflösung](/assets/euler/de/II-I-2.pdf)