---
layout: page
title: Chapter 2. "Of Arithmetical Proportion."
part: I
section: III
chapter: 2
---

### Part {{ page.part }}. Section {{ page.section }}. {{ page.title }}

<span class="art">390</span> When two arithmetical ratios, or relations, are equal,
this equality is called an **arithmetical proportion**.

Thus, when $$a - b = d$$ and $$p - q = d$$, so that the difference is the same between the numbers $$p$$ and $$q$$ as between
the numbers $$a$$ and $$b$$, we say that these four numbers form
an arithmetical proportion; which we write thus, $$a - b = p - q$$, expressing clearly by this, that the difference between
$$a$$ and $$b$$ is equal to the difference between $$p$$ and $$q$$.

<span class="art">391</span> An arithmetical proportion consists therefore of four
terms, which must be such, that if we subtract the second
from the first, the remainder is the same as when we subtract the fourth from the third; thus, the four numbers 12, 7, 9, 4,
form an arithmetical proportion, because 12 - 7 = 9 - 4.

<span class="art">392</span> When we have an arithmetical proportion, as $$a - b = p - q$$, we may make the second and third terms change
places, writing $$a - p = b - q$$: and this equality will be
no less true; for, since $$a - b = p - q$$, add $$b$$ to both sides,
and w have $$a = b + p - q$$: then subtract $$p$$ from both
sides, and we have $$a - p = b - q$$.
In the same manner, as 12 - 7 = 9 - 4, so also 12 - 9 = 7 - 4.

<span class="art">393</span> We may in every arithmetical proportion put the
second term also in the place of the first, if we make the
same transposition of the third and fourth; that is, if
$$a - b = p - q$$, we have also $$b - a = q - p$$; for $$b - a$$ is
the negative of $$a-b$$, and $$q - p$$ is also the negative of
$$p - q$$; and thus, since 12 - 7 = 2 - 4, we have also,
7 - 12 = 4 - 9.

<span class="art">394</span> But the most interesting property of every arithmetical proportion is this, that the sum of the second and
third term is always equal to the sum of the first and fourth.
This property, which we must particularly consider, is expressed also by saying that the sum of the *means* is equal
to the sum of the *extremes*. Thus, since 12 - 7 = 9 - 4,
we have 7 + 9 = 12 + 4; the sum being in both cases 16.

<span class="art">395</span> In order to demonstrate this principal property, let
$$a - b=p - q$$; then if we add to both $$b+q$$, we have
$$a + q = b + p$$; that is, the sum of the first and fourth
terms is equal to the sum of the second and third: and inversely, of four numbers, $$a$$, $$b$$, $$p$$, $$q$$, are such, that the sum
of the second and third is equal to the sum of the first and
fourth; that is, if $$b + p = a + q$$, we conclude, without a
possibility of mistake, that those numbers are in arithmetical
proportion, and that $$a - b = p - q$$; for, since $$a + q = b + p$$,
if we subtract from both sides $$b + q$$, we obtain $$a - b = p - q$$.

Thus, the numbers 18, 13, 15, 10, being such, that the
sum of the means (13+15=28) is equal to the sum of
the extremes (18+10=28), it is certain that they also
form an arithmetical proportion; and, consequently, that
18 - 13 = 15 - 10.

<span class="art">396</span> It is easy, by means of this property, to resolve the
following question. The first three terms of an arithmetical
proportion being given, to find the fourth? Let $$a$$, $$b$$, $$p$$, be
the first three terms, and let us express the fourth by $$q$$,
which it is required to determine, then $$a + q = b + p$$; by
subtracting $$a$$ from both sides, we obtain $$q = b + p - a$$.

Thus, the fourth term is found by adding together the
second and third, and subtracting the first from that sum.
Suppose, for example, that 19, 28, 13, are the three first
given terms, the sum of the second and third is 41; and
taking from it the first, which is 19, there remains 22 for the
fourth term sought, and the arithmetical proportion will be
represented by 19 - 28 = 13 - 22, or by 28 - 19 = 22 - 13, or, lastly,
by 28 - 22 = 19 - 13.

<span class="art">397</span> When in arithmetical proportion the second term is
equal to the third, we have only three numbers; the property of which is this, that the first, minus the second, is
equal to the second, minus the third; or that the difference
between the first and second number is equal to the difference between the second and third: the three numbers
19, 15, 11, are of this kind, since 19 - 15 = 15 - 11.

<span class="art">398</span> Three such numbers are said to form a continued
arithmetical proportion, which is sometimes written thus,
19:15:11. Such proportions are also called **arithmetical progressions**, particularly if a greater number of terms
follow each other according to the same law.

An arithmetical progression may be either increasing, or
decreasing. The former distinction is applied when the
terms go on increasing; that is to say, when the second exceeds the first, and the third exceeds the second by the
same quantity; as in the numbers 4, 7, 10; and the decreasing progression is that in which the terms go on always
diminishing by the same quantity, such as the numbers 9, 5, 1.

<span class="art">399</span> Let us suppose the numbers $$a$$, $$b$$, $$c$$, to be in arithmetical progression; then $$a - b = b - c$$, whence it follows,
from the equality between the sum of the extremes and that
of the means, that $$2b = a + c$$; and if we subtract a from
both, we have $$2b - a = c$$.

<span class="art">400</span> So that when the first two terms $$a$$, $$b$$, of an arithmetical progression are given, the third is found by taking
the first from twice the second. Let 1 and 3 be the first
two terms of an arithmetical progression, the third will be
2·3 - 1 = 5; and these three numbers 1, 3, 5, give the proportion

1 - 3 = 3 - 5.

<span class="art">401</span> By following the same method, we may pursue the
arithmetical progression as far as we please ; we have only
to find the fourth term by means of the second and third,
in the same manner as we determined the third by means of
the first and second, and so on. Let $$a$$ be the first term, and
$$b$$ the second, the third will be $$2b - a$$, the fourth $$4b - 2a - b = 3b - 2a$$, the fifth $$6b - 4a - 2b + a = 4b - 3a$$,
the sixth $$8b - 6a - 3b + 2a = 5b - 4a$$, the seventh
$$10b - 8a - 4b + 3a = 6b - 5a$$, etc.

#### Editions

1. Leonhard Euler. *Elements of Algebra*. Translated by Rev. John Hewlett. Third Edition. Longmans, Hurst, Rees, Orme, and Co. London. 1822.
    - [Part {{ page.part }}. Section {{ page.section }}. {{ page.title }}](/EulerAlgebra/en/III-2.pdf)
2. Leonhard Euler. *Vollständige Anleitung zur Algebra. Mit den Zusätzen von Joseph Louis Lagrange.* Herausgegeben von Heinrich Weber. B. G. Teubner. Leipzig and Berlin. 1911. Leonhardi Euleri Opera omnia. Series prima. Opera mathematica. Volumen primum.
    - [Erster Theil. Dritter Abschnitt. Capitel 2. Von den arithmetischen Proportionen](/EulerAlgebra/de/I-III-2.pdf)