---
layout: page
title: Chapter 6. "Of the Cases in Integer Numbers, in which the Formula ùëéùë•ùë•+ùëè becomes a Square."
part: II
chapter: 6
---

### Part {{ page.part}}. {{ page.title }}

<span class="art">79</span> We have already shown, <span class="artref">Art. 63</span>, how such formulae
as $$a+bx+cx^2$$ are to be transformed, in order that the
second term may be destroyed  we shall therefore confine
our present inquiries to the formula $$ax^2 + b$$, in which it is
required to find for $$x$$ only integer numbers, which may
transform that formula into a square. Now, first of all,
such a formula must be possible; for, if it be not, we shall
not even obtain fractional values of $$x$$, far less integer ones.

<span class="art">80</span> Let us suppose then $$ax^2+b=y^2$$; $$a$$ and $$b$$ being
integer numbers, as well as $$x$$ and $$y$$.

Now, here it is absolutely necessary for us to know, or to
have already found a case in integer numbers; otherwise it
would be lost labor to seek for other similar cases, as the
formula might happen to be impossible.

We shall, therefore, suppose that this formula becomes a
square, by making $$x-f$$, and we shall represent that square
by $$g^2$$, so that $$af^2+b=g^2$$, where $$f$$ and $$g$$ are known
numbers. Then we have only to deduce from this case other similar
cases; and this inquiry is so much the more important,
as it is subject to considerable difficulties; which,
however, we shall be able to surmount by particular artifices.

<span class="art">81</span> Since we have already found $$af^2+b=g^2$$,
and likewise, by hypothesis, $$ax^2+b=y^2$$,
let us subtract the first
equation from the second, and we shall obtain a new one,
$$ax^2-af^2=y^2-g^2$$, which may be represented by factors
in the following manner;

$$a(x+f)\cdot(x-f) = (y+g)\cdot (y-g),$$

and which, by multiplying both sides by $$pq$$, becomes

$$apq(x+f)\cdot(x-f)=pq(y+g)\cdot(y-g).$$

If we now decompound this equation, by making $$ap(x+f)=q(y+g)$$,
and $$q(x-f) = p(y-g)$$, we may derive, from
these two equations, values of the two letters $$x$$ and $$y$$. The
first, divided by $$q$$, gives $$y+g = \dfrac{apx+apf}{q}$$;
and the second, divided by $$p$$, gives $$y-g = \dfrac{qx-qf}{p}$$.
Subtracting this
latter equation from the former, we have

$$2g = \dfrac{(ap^2-q^2)x+(ap^2+q^2)f}{pq},$$

or

$$2gpq = (ap^2-q^2)x+(ap^2+q^2)f;$$

therefore

$$x=\dfrac{2gpq}{ap^2-q^2} - \dfrac{(ap^2+q^2)f}{ap^2-q^2},$$

from which we obtain

$$y=g+\dfrac{2gq^2}{ap^2-q^2} - \dfrac{(ap^2+q^2)fq}{(ap^2-q^2)p} - \dfrac{qf}{p}.$$

And as, in this latter value, the first two terms, both containing the letter $$g$$,
may be put into the form $$\dfrac{g(ap^2+q^2)}{ap^2-q^2}$$, and as the other two,
containing the letter $$f$$, may be expressed by $$\dfrac{2afpq}{ap^2-q^2}$$,
all the
terms will be reduced to the same denomination, and we
shall have

$$y=\dfrac{g(ap^2+q^2)-2afpq}{ap^2-q^2}.$$

<span class="art">82</span> This operation seems not, at first, to answer our purpose;
since having to find integer values of $$x$$ and $$y$$, we are
brought to fractional results; and it would be required to
solve this new question, - What numbers are we to substitute
for $$p$$ and $$q$$, in order that the fraction may disappear? A
question apparently still more difficult than our original one:
but here we may employ a particular artifice, that will
readily bring us to our object, which is as follows:

As every thing must be expressed in integer numbers, let
us make $$\dfrac{ap^2+q^2}{ap^2-q^2}=m$$, and $$\dfrac{2pq}{ap^2-q^2}=n$$,
in order that we may have $$x=ng-mf$$, and $$y=mg-naf$$.

Now, we cannot here assume $$m$$ and $$n$$ at pleasure, since
these letters must be such as will answer to what has been
already determined: therefore, for this purpose, let us consider their squares, and we shall find

$$m^2=\dfrac{a^2p^4+2ap^2q^2+q^4}{a^2p^4-2ap^2q^2+q^4},$$

and

$$n^2=\dfrac{4p^2q^2}{a^2p^4-2ap^2q^2+q^4};$$

and hence

$$
\begin{align}
m^2-an^2&=\dfrac{a^2p^4+2ap^2q^2+q^4-4ap^2q^2}{a^2p^4-2ap^2q^2+q^4}\\
&=\dfrac{a^2p^4-2ap^2q^2+q^4}{a^2p^4-2ap^2q^2+q^4}\\
&=1.
\end{align}
$$

<span class="art">83</span> We see, therefore, that tlie two numbers $$m$$ and $$n$$
must be such, that $$m^2=an^2+1$$. So that, as $$a$$ is a known
number, we must begin by considering the means of determining such an integer number for $$n$$,
as will make
$$an^2+1$$ a square; for then $$m$$ will be the root of that square;
and when we have likewise determined the number $$f$$ so,
that $$af^2+b$$ may become a square, namely $$g^2$$ we shall obtain for $$x$$ and $$y$$
the following values in integer numbers;

$$x=ng-mf,\qquad y =mg-naf;$$

and thence, lastly, $$ax^2+b=y^2$$.

<span class="art">84</span> It is evident, that having once determined $$m$$ and $$n$$,
we may write instead of them $$-m$$ and $$-n$$, because the
square $$n^2$$ still remains the same.

But we have already shewn that, in order to find $$x$$ and $$y$$
in integer numbers, so that $$ax^2+b=y^2$$, we must first
know a case, such that $$af^2+b$$ may be equal to $$g^2$$; when
we have therefore found such a case, we must also endeavour
to know, beside the number $$a$$, the values of $$m$$ and $$n$$, which
will give $$an^2+1=m^2$$: the method for which shall be described in the sequel,
and when this is done, we shall have a
new case, namely, $$x=ng+mf$$, and $$y=mg+naf$$, also $$ax^2+b=y^2$$.

Putting this new case instead of the preceding one, which
was considered as known; that is to say, writing $$ng + mf$$
for $$f$$, and $$mg + naf$$ for $$g$$, we shall have new values of $$x$$
and $$y$$, from which, if they be again substituted for $$x$$ and $$y$$,
we may find as many other new values as we please: so
that, by means of a single case known at first,
we mav afterwards determine an infinite number of others.

<span class="art">85</span> The manner in which we have arrived at this solution
has been very embarrassed, and seemed at first to lead us
from our object, since it brought us to complicated fractions,
which an accidental circumstance only enabled us to reduce:
it will be proper, therefore, to explain a shorter method,
which leads to the same solution.

<span class="art">86</span> Since we must have $$ax^2+b=y^2$$, and have already found
$$af^2+b=g^2$$, the first equation gives us
$$b=y^2-ax^2$$, and the second gives $$b=g^2-af^2$$;
consequently, also, $$y^2-ax^2=g^2-af^2$$, and the whole is reduced
to determining the unknown quantities $$x$$ and $$y$$, by means
of the known quantities $$f$$ and $$g$$. It is evident, that for this purpose,
we need only make $$x=f$$ and $$y=g$$;
but it is also
evident, that this supposition would not furnish a new case
in addition to that already known. We shall, therefore,
suppose that we have already found such a number for $$n$$,
that $$an^2+1$$ is a square, or that $$an^2+1=m^2$$; which being
laid down, we have $$m^2-an^2=1$$; and multiplying by this equation
the one we had last, we find also

$$y^2-ax^2=(g^2-af^2)\cdot(m^2-an^2) = g^2m^2-af^2m^2-ag^2n^2+a^2f^2n^2.$$

Let us now suppose $$y=gm+afn$$, and we shall have

$$g^2m^2+2afgmn+a^2f^2n^2-ax^2=g^2m^2-af^2m^2-ag^2n^2+a^2f^2n^2,$$

in which the terms $$g^2m^2$$ and $$a^2f^2m^2$$ are destroyed; so that
there remains $$ax^2=af^2m^2+ag^2n^2+2afgmn$$, or
$$x^2=f^2m^2+2fgmn+g^2n^2$$.
Now, this formula is evidently a
square, and gives $$x=fm+gn$$. Hence we have obtained
the same formulae for $$x$$ and $$y$$ as before.

<span class="art">87</span> It will be necessary to render this solution more
evident, by applying it to some examples.

*Question 1.* To find all the integer values of $$x$$, that
will make $$2x^2-1$$, a square, or give $$2x^2-1=y^2$$.

Here, we have $$a=2$$ and $$b=-1$$; and a satisfactory


case immediately presents itself, namely, that in which $$x=1$$
and $$y=1$$: which gives $$f=1$$ and $$g=1$$. Now, it is
farther required to determine such a value of $$n$$, as will give
$$2n^2+1=m^2$$; and we see immediately, that this obtains
when $$n=2$$, and consequently $$m=3$$; so that every case,
which is known for $$f$$ and $$g$$, giving us these new cases
$$x=3f+2g$$, and $$y=3g+4f$$, we derive from the first
solution, $$f=1$$ and $$g=1$$, the following new solutions:

$$
\begin{array}{r|r|r|r}
x=f=1&5&29&169\\
y=g=1&7&41&239, \; \textrm{etc.}
\end{array}
$$

<span class="art">88</span> *Question 2.* To find all the triangular numbers,
that are at the same time squares.

Let $$z$$ be the triangular root; then
$$\dfrac{z^2+z}{2}$$ is the triangle, which is to be also a square;
and if we call $$x$$ the root  of this square, we have
$$\dfrac{z^2+z}{2}=x^2$$: multiplying by 8, we have
$$4z^2+4z=8x^2$$; and also adding 1 to each side, we have

$$4z^2+4z+1=(2z+1)^2=8x^2-1.$$

Hence the question is to make $$8x^2+1$$ become a square;
for, if we find $$8x^2+1=y^2$$, we shall have $$y=2z+1$$,
and, consequently, the triangular root will be

$$z=\dfrac{y-1}{2}.$$

Now, we have $$a=8$$, and $$b=1$$, and a satisfactory case immediately
occurs, namely, $$f=0$$ and $$g=1$$. It is farther evident, that
$$8n^2+1=m^2$$, and if we make $$n=1$$, and $$m=3$$;
therefore $$x=3f+g$$, and $$y=3g+8f$$; and since
$$z=\dfrac{y-1}{2}$$, we shall have the following solutions:

$$
\begin{array}
x=f=0&1&6&35&204&1189\\
y=g=1&3&17&99&577&3363\\
z=\frac{y-1}{2}=0&1&8&49&288&1681,\;\textrm{etc.}
\end{array}
$$

<span class="art">89</span> *Question 3.* To find all the pentagonal numbers,
which are at the same time squares.

If the root be $$z$$, the pentagon will be $$=\dfrac{3z^2-z}{2}$$, which
we shall make equal to $$x^2$$, so that $$3z^2-z=2x^2$$;
then multiplying by 12, and adding unity, we have

$$36z^2-12z+1 = (6z-1)^2 = 24x^2+1;$$

also, making $$24x^2+1=y^2$$, we have $$y=6z-1$$, and $$z=\dfrac{y+1}{6}$$.

Since $$a=24$$, and $$b=1$$, we know the case $$f=0$$, and $$g=1$$;
and as we must have $$24n^2+1=m^2$$, we shall make
$$n=1$$, which gives $$m=5$$; so that we shall have $$x=5f+g$$
and $$y=5g+24f$$; and not only $$z=\dfrac{y+1}{y}$$, but also
$$z=\dfrac{1-y}{6}$$, because we may write $$y=1-6z$$: whence we
find the following results:

$$
\begin{array}{r|r|r|r|r}
x=f=0&1&10&99&980\\
y=g=1&5&49&485&4801\\
z=\dfrac{y+1}{6}=\frac{1}{3}&1&\frac{25}{3}&81&\frac{2401}{3}\\
\textrm{or} \quad z=\dfrac{1-y}{6}=0&-\frac{2}{3}&-8&-\frac{242}{8}&-800, \; \textrm{etc.}
\end{array}
$$

<span class="art">90</span>




<span class="art">91</span>

#### Editions

1. Leonhard Euler. *Elements of Algebra*. Translated by Rev. John Hewlett. Third Edition. Longmans, Hurst, Rees, Orme, and Co. London. 1822.
    - [Part {{ page.part}}. {{ page.title }}](/assets/euler/en/pt-II-6.pdf)
2. Leonhard Euler. *Vollst√§ndige Anleitung zur Algebra. Mit den Zus√§tzen von Joseph Louis Lagrange.* Herausgegeben von Heinrich Weber. B. G. Teubner. Leipzig and Berlin. 1911. Leonhardi Euleri Opera omnia. Series prima. Opera mathematica. Volumen primum.
    - [Zweyter Theil. Zweyter Abschnitt. Capitel 6. Von den F√§llen in gantzen Zahlen, da die Formel $$axx + b$$ ein Quadrat wird](/assets/euler/de/II-II-6.pdf)